SporkProofs/Semantics.lean
@@ -1,142 +1,10 @@
 import SporkProofs.Syntax
 
-theorem congrArg₂ {α β γ} (f : α → β → γ) {x x' : α} {y y' : β}
-    (hx : x = x') (hy : y = y') : f x y = f x' y' := by subst hx hy; rfl
-
--- TODO: inlining of nested parreduces!!
-
 abbrev ValMap : Type := List Val
-
-instance instValMapGetElem : GetElem ValMap Var Val (λ X x => x.Okay X.length) where
-  getElem X x xₒₖ := X[x.idx]'xₒₖ.1
-
-instance instValMapGetElems : GetElem ValMap (List Var) (List Val) (λ X => IVec (·.Okay X.length)) where
-  getElem X _args argsₒₖ := argsₒₖ.map (λ x xₒₖ => X[x])
-
-abbrev valOf (p : Prop) [d : Decidable p] : Val := if decide p then 1 else 0
-
-namespace Atom
-  abbrev eval : (X : ValMap) -> (a : Atom) -> (a.Okay X.length) -> Val
-    | _X, .val v, _okᵥ => v
-    | X, .var x, okₓ =>
-      let _ := match okₓ with | .var p => p
-      X[x]
-
-  inductive Eval (X : ValMap) (a : Atom) : Val -> Prop where
-    | mk (okₐ : a.Okay X.length) : Eval X a (eval X a okₐ)
-
-  notation (name := atomeval) X:arg " ⊢ₐₜₒₘ " a:arg " ⇓ " v:arg => Eval X a v
-
-  namespace Eval
-    instance instDecidableEval : {X : ValMap} -> {a : Atom} -> {v : Val} -> Decidable (X ⊢ₐₜₒₘ a ⇓ v)
-      | X, a, v => decidable_of_iff (∃ p : a.Okay X.length, eval X a p = v)
-        ⟨λ ⟨okₐ, p⟩ => p ▸ Eval.mk okₐ,
-         λ | (Eval.mk okₐ) => ⟨okₐ, rfl⟩⟩
-
-    theorem okay {X : ValMap} {a : Atom} {v : Val} : Eval X a v -> a.Okay X.length
-      | Eval.mk okₐ => okₐ
-    theorem eq {X : ValMap} {a : Atom} {v : Val} : (s : Eval X a v) -> eval X a (okay s) = v
-      | Eval.mk okₐ => rfl
-
-    abbrev progress (X : ValMap) (a : Atom) (okₐ : a.Okay X.length) : Σ' v, Eval X a v :=
-      ⟨eval X a okₐ, Eval.mk okₐ⟩
-  end Eval
-end Atom
-
-namespace Bop
-  abbrev eval : Bop -> Val -> Val -> Val
-    | .IADD, u, v => u + v
-    | .ISUB, u, v => u - v
-    | .IMUL, u, v => u * v
-    | .IDIV, u, v => u / v
-    | .IMOD, u, v => u % v
-    | .ILT,  u, v => valOf (u < v)
-    | .ILE,  u, v => valOf (u ≤ v)
-    | .IGT,  u, v => valOf (u > v)
-    | .IGE,  u, v => valOf (u ≥ v)
-    | .IEQ,  u, v => valOf (u = v)
-    | .INE,  u, v => valOf (u ≠ v)
-    | .LAND, u, v => valOf (u ≠ 0 && v ≠ 0)
-    | .LOR,  u, v => valOf (u ≠ 0 || v ≠ 0)
-    | .LXOR, u, v => valOf (u ≠ 0 ^^ v ≠ 0)
-
-  inductive Eval (o : Bop) (u v : Val) : Val -> Prop where
-    | mk : Eval o u v (eval o u v)
-
-  namespace Eval
-    instance instDecidable {o : Bop} {u v w : Val} : Decidable (Eval o u v w) :=
-      decidable_of_iff (eval o u v = w)
-        ⟨λ p => p ▸ Eval.mk,
-         λ | Eval.mk => rfl⟩
-
-    theorem eq {o : Bop} {u v w : Val} : Eval o u v w -> eval o u v = w
-      | Eval.mk => rfl
-
-    abbrev progress (o : Bop) (u v : Val) : Σ' w, Eval o u v w :=
-      ⟨eval o u v, Eval.mk⟩
-  end Eval
-end Bop
-
-namespace Uop
-  abbrev eval : Uop -> Val -> Val
-    | INEG, v => -v
-    | LNOT, v => valOf (v = 0)
-
-  inductive Eval (o : Uop) (v : Val) : Val -> Prop where
-    | mk : Eval o v (eval o v)
-
-  namespace Eval
-    instance instDecidable {o : Uop} {u v : Val} : Decidable (Eval o u v) :=
-      decidable_of_iff (eval o u = v)
-        ⟨λ p => p ▸ Eval.mk,
-         λ | Eval.mk => rfl⟩
-
-    theorem eq {o : Uop} {u v : Val} : Eval o u v -> eval o u = v
-      | Eval.mk => rfl
-
-    abbrev progress (o : Uop) (u : Val) : Σ' v, Eval o u v :=
-      ⟨eval o u, Eval.mk⟩
-  end Eval
-end Uop
-
-namespace Expr
-  abbrev eval (X : ValMap) : (e : Expr) -> (e.Okay X.length) -> Val
-    | nop a, ok =>
-      let aₒₖ := match ok with | .nop aₒₖ => aₒₖ
-      a.eval X aₒₖ
-    | uop o a, ok =>
-      let aₒₖ := match ok with | .uop aₒₖ => aₒₖ
-      o.eval (a.eval X aₒₖ)
-    | bop o a b, ok =>
-      let aₒₖ := match ok with | .bop aₒₖ _ => aₒₖ
-      let bₒₖ := match ok with | .bop _ bₒₖ => bₒₖ
-      o.eval (a.eval X aₒₖ) (b.eval X bₒₖ)
-
-  inductive Eval (X : ValMap) (e : Expr) : Val -> Prop where
-    | mk (eₒₖ : e.Okay X.length) : Eval X e (eval X e eₒₖ)
-
-  notation (name := expreval) X:arg " ⊢ₑₓₚᵣ " e:arg " ⇓ " v:arg => Eval X e v
-
-  namespace Eval
-    instance instDecidable {X : ValMap} {e : Expr} {v : Val} : Decidable (X ⊢ₑₓₚᵣ e ⇓ v) :=
-      decidable_of_iff (∃ (eₒₖ : e.Okay X.length), eval X e eₒₖ = v)
-        ⟨λ ⟨eₒₖ, p⟩ => p ▸ mk eₒₖ,
-         λ | mk eₒₖ => ⟨eₒₖ, rfl⟩⟩
-
-    theorem okay {X : ValMap} {e : Expr} {v: Val} : X ⊢ₑₓₚᵣ e ⇓ v -> e.Okay X.length
-      | mk eₒₖ => eₒₖ
-    theorem eq  {X : ValMap} {e : Expr} {v: Val} : (s : X  ⊢ₑₓₚᵣ e ⇓ v) -> eval X e (okay s) = v
-      | mk eₒₖ => rfl
-
-    abbrev progress (X : ValMap) (e : Expr) (eₒₖ : e.Okay X.length) : Σ' v, X  ⊢ₑₓₚᵣ e ⇓ v :=
-      ⟨eval X e eₒₖ, Eval.mk eₒₖ⟩
-  end Eval
-end Expr
 
 inductive StackFrameCode : Type
   | code (c : Code)
   | cont (b : Cont)
--- open StackFrameCode code cont
 
 inductive SpawnCall : Type where
   | mk (f : FuncIdx) (args : List Val) (ret : Nat)
@@ -156,20 +24,141 @@ inductive CallStack : Type where
   | nil
   | cons (K : CallStack) (k : StackFrame)
 
-inductive ThreadPool : Type where
-  | leaf : CallStack -> ThreadPool
-  | cat : ThreadPool -> ThreadPool -> ThreadPool
+inductive ThreadTree : Type where
+  | thread : CallStack -> ThreadTree
+  | node : ThreadTree -> ThreadTree -> ThreadTree
 
-namespace StackFrameCode
-  -- instance instCoeToSum : Coe (Code ⊕ Cont) StackFrameCode where
-  --   coe := Sum.elim code cont
-  -- instance instCoeFmSum : Coe StackFrameCode (Code ⊕ Cont) where
-  --   coe := fun | code c => Sum.inl c | cont k => Sum.inr k
-  
+
+namespace ValMap
+  instance : GetElem ValMap Var Val (λ X x => x.WF X.length) where
+    getElem X x xwf := X[x.idx]'xwf.1
+
+  instance : GetElem ValMap (List Var) (List Val) (λ X => IVec (·.WF X.length)) where
+    getElem X _args argswf := argswf.list_map (λ x xwf => X[x])
+end ValMap
+
+@[simp] def valOf (p : Prop) [d : Decidable p] : Val := if decide p then 1 else 0
+
+namespace Atom
+  @[simp] def eval : (X : ValMap) -> (a : Atom) -> a.WF X.length -> Val
+    | _X, .val v, _wfᵥ => v
+    | X, .var x, wfₓ =>
+      let _ := match wfₓ with | .var p => p
+      X[x]
+
+  inductive Eval (X : ValMap) (a : Atom) : Val -> Prop where
+    | mk (wfₐ : a.WF X.length) : Eval X a (eval X a wfₐ)
+
+  notation (name := atomeval) X:arg " ⊢ₐₜₒₘ " a:arg " ⇓ " v:arg => Eval X a v
+
+  namespace Eval
+    instance : {X : ValMap} -> {a : Atom} -> {v : Val} -> Decidable (X ⊢ₐₜₒₘ a ⇓ v)
+      | X, a, v => decidable_of_iff (∃ p : a.WF X.length, eval X a p = v)
+        ⟨λ ⟨wfₐ, p⟩ => p ▸ Eval.mk wfₐ,
+         λ | (Eval.mk wfₐ) => ⟨wfₐ, rfl⟩⟩
+
+    theorem wf {X : ValMap} {a : Atom} {v : Val} : Eval X a v -> a.WF X.length
+      | Eval.mk wfₐ => wfₐ
+    theorem eq {X : ValMap} {a : Atom} {v : Val} : (s : Eval X a v) -> eval X a (wf s) = v
+      | Eval.mk wfₐ => rfl
+  end Eval
+end Atom
+
+namespace Bop
+  @[simp] def eval : Bop -> Val -> Val -> Val
+    | .IADD, u, v => u + v
+    | .ISUB, u, v => u - v
+    | .IMUL, u, v => u * v
+    | .IDIV, u, v => u / v
+    | .IMOD, u, v => u % v
+    | .ILT,  u, v => valOf (u < v)
+    | .ILE,  u, v => valOf (u ≤ v)
+    | .IGT,  u, v => valOf (u > v)
+    | .IGE,  u, v => valOf (u ≥ v)
+    | .IEQ,  u, v => valOf (u = v)
+    | .INE,  u, v => valOf (u ≠ v)
+    | .LAND, u, v => valOf (u ≠ 0 && v ≠ 0)
+    | .LOR,  u, v => valOf (u ≠ 0 || v ≠ 0)
+    | .LXOR, u, v => valOf (u ≠ 0 ^^ v ≠ 0)
+
+  inductive Eval (o : Bop) (u v : Val) : Val -> Prop where
+    | mk : Eval o u v (eval o u v)
+
+  namespace Eval
+    instance {o : Bop} {u v w : Val} : Decidable (Eval o u v w) :=
+      decidable_of_iff (eval o u v = w)
+        ⟨λ p => p ▸ Eval.mk,
+         λ | Eval.mk => rfl⟩
+
+    theorem eq {o : Bop} {u v w : Val} : Eval o u v w -> eval o u v = w
+      | Eval.mk => rfl
+  end Eval
+end Bop
+
+namespace Uop
+  @[simp] def eval : Uop -> Val -> Val
+    | INEG, v => -v
+    | LNOT, v => valOf (v = 0)
+
+  inductive Eval (o : Uop) (v : Val) : Val -> Prop where
+    | mk : Eval o v (eval o v)
+
+  namespace Eval
+    instance {o : Uop} {u v : Val} : Decidable (Eval o u v) :=
+      decidable_of_iff (eval o u = v)
+        ⟨λ p => p ▸ Eval.mk,
+         λ | Eval.mk => rfl⟩
+
+    theorem eq {o : Uop} {u v : Val} : Eval o u v -> eval o u = v
+      | Eval.mk => rfl
+  end Eval
+end Uop
+
+namespace Expr
+  @[simp] def eval (X : ValMap) : (e : Expr) -> (e.WF X.length) -> Val
+    | nop a, wf =>
+      let awf := match wf with | .nop awf => awf
+      a.eval X awf
+    | uop o a, wf =>
+      let awf := match wf with | .uop awf => awf
+      o.eval (a.eval X awf)
+    | bop o a b, wf =>
+      let awf := match wf with | .bop awf _ => awf
+      let bwf := match wf with | .bop _ bwf => bwf
+      o.eval (a.eval X awf) (b.eval X bwf)
+
+  inductive Eval (X : ValMap) (e : Expr) : Val -> Prop where
+    | mk (ewf : e.WF X.length) : Eval X e (eval X e ewf)
+
+  notation (name := expreval) X:arg " ⊢ₑₓₚᵣ " e:arg " ⇓ " v:arg => Eval X e v
+
+  namespace Eval
+    instance {X : ValMap} {e : Expr} {v : Val} : Decidable (X ⊢ₑₓₚᵣ e ⇓ v) :=
+      decidable_of_iff (∃ (ewf : e.WF X.length), eval X e ewf = v)
+        ⟨λ ⟨ewf, p⟩ => p ▸ mk ewf,
+         λ | mk ewf => ⟨ewf, rfl⟩⟩
+
+    theorem wf {X : ValMap} {e : Expr} {v: Val} : X ⊢ₑₓₚᵣ e ⇓ v -> e.WF X.length
+      | mk ewf => ewf
+    theorem eq  {X : ValMap} {e : Expr} {v: Val} : (s : X  ⊢ₑₓₚᵣ e ⇓ v) -> eval X e (wf s) = v
+      | mk ewf => rfl
+  end Eval
+end Expr
+
+theorem codeOfGetElem {P : Program} {f : FuncIdx} {b : Cont}
+                    (pf : f < P.size) (pb : b.b < P[f].size) :
+                    P[f]![b.b]! = P[f][b.b] :=
+  by rw[getElem!_pos P f pf, getElem!_pos P[f] b.b pb]
+
+theorem argsOfGetElem {x : List Var} {X : ValMap} (wf : IVec (·.WF X.length) x):
+                    X[x]! = X[x] :=
+  getElem!_pos X x wf
+
+namespace StackFrameCode  
   abbrev isCode | code _ => true | cont _ => false
   abbrev isCont | code _ => false | cont _ => true
 
-  abbrev extractD : (c : StackFrameCode) -> if isCode c then Code else Cont
+  @[simp] def extractD : (c : StackFrameCode) -> if isCode c then Code else Cont
     | code c => c
     | cont b => b
   abbrev extractCode : (c : StackFrameCode) -> isCode c -> Code
@@ -177,77 +166,66 @@ namespace StackFrameCode
   abbrev extractCont : (c : StackFrameCode) -> isCont c -> Cont
     | cont b, _ => b
 
-  inductive Okay (fsigs bsigs bsig ret) : StackFrameCode -> Prop
-    | code {c} : c.Okay fsigs bsigs ret bsig -> (code c).Okay fsigs bsigs bsig ret
-    | cont {b} : b.OkayRets bsigs bsig ret -> (cont b).Okay fsigs bsigs bsig ret
+  @[simp] abbrev codeOf (P : Program) (f : FuncIdx) (b : Cont) : StackFrameCode :=
+    code P[f]![b.b]!.code
+  @[simp] abbrev codeEntry (P : Program) (f : FuncIdx) : StackFrameCode :=
+    code P[f]!.blocks.head!.code
 
-  namespace Okay
-    abbrev c {fsigs bsigs bsig ret c} :
-             Okay fsigs bsigs bsig ret (.code c) ->
-             c.Okay fsigs bsigs ret bsig
+  inductive WF (fsigs bsigs bsig ret) : StackFrameCode -> Prop
+    | code {c} : c.WF fsigs bsigs ret bsig -> (code c).WF fsigs bsigs bsig ret
+    | cont {b} : b.WFRets bsigs bsig ret -> (cont b).WF fsigs bsigs bsig ret
+
+  namespace WF
+    instance {fsigs bsigs bsig ret} : (c : StackFrameCode) ->
+             Decidable (c.WF fsigs bsigs bsig ret)
+      | .code c =>
+        decidable_of_iff (c.WF fsigs bsigs ret bsig)
+          ⟨code, λ (code p) => p⟩
+      | .cont b =>
+        decidable_of_iff (b.WFRets bsigs bsig ret)
+          ⟨cont, λ (cont p) => p⟩
+
+    theorem c {fsigs bsigs bsig ret c} :
+             WF fsigs bsigs bsig ret (.code c) ->
+             c.WF fsigs bsigs ret bsig
       | code c => c
 
-    abbrev b {fsigs bsigs bsig b ret} :
-             Okay fsigs bsigs bsig ret (.cont b) ->
-             b.OkayRets bsigs bsig ret
+    theorem b {fsigs bsigs bsig b ret} :
+             WF fsigs bsigs bsig ret (.cont b) ->
+             b.WFRets bsigs bsig ret
       | cont b => b
-  end Okay
+  end WF
 
-  instance instDecidable {fsigs bsigs bsig ret} :
-                         (c : StackFrameCode) ->
-                         Decidable (c.Okay fsigs bsigs bsig ret)
-    | code c =>
-      decidable_of_iff (c.Okay fsigs bsigs ret bsig)
-        ⟨Okay.code, λ | Okay.code p => p⟩
-    | cont b =>
-      decidable_of_iff (b.OkayRets bsigs bsig ret)
-        ⟨Okay.cont, λ | Okay.cont p => p⟩
-
-  -- instance instDecidableEq : DecidableEq StackFrameCode
-  --   | code c, code c' =>
-  --     decidable_of_iff (c = c')
-  --       ⟨congrArg code, congrArg (λ | code c => c | _ => c)⟩
-  --   | cont b, cont b' =>
-  --     decidable_of_iff (b = b')
-  --       ⟨congrArg cont, congrArg (λ | cont b => b | _ => b)⟩
-  --   | code c, cont b => isFalse (by simp)
-  --   | cont b, code c => isFalse (by simp)
   deriving instance DecidableEq for StackFrameCode
 end StackFrameCode
 
 namespace SpawnCall
-  abbrev f | mk f _args _ret => f
-  abbrev args | mk _f args _ret => args
-  abbrev ret | mk _f _args ret => ret
+  @[simp] abbrev f | mk f _args _ret => f
+  @[simp] abbrev args | mk _f args _ret => args
+  @[simp] abbrev ret | mk _f _args ret => ret
 
-  inductive Okay (fsigs : FuncSigs) (sc : SpawnCall) : Prop where
+  inductive WF (fsigs : FuncSigs) (sc : SpawnCall) : Prop where
     | mk (_ : sc.f < fsigs.length)
          (_ : ⟨sc.args.length, sc.ret⟩ = fsigs[sc.f]) :
-         sc.Okay fsigs
+         sc.WF fsigs
 
-  namespace Okay
-    abbrev flt {fsigs} {sc : SpawnCall} : sc.Okay fsigs -> sc.f < fsigs.length | mk flt _ => flt
-    abbrev sig {fsigs} {sc : SpawnCall} : (ok : sc.Okay fsigs) -> ⟨sc.args.length, sc.ret⟩ = fsigs[sc.f]'ok.flt | mk _ sig => sig
-  end Okay
+  namespace WF
+    instance {fsigs : FuncSigs} : (sc : SpawnCall) -> Decidable (sc.WF fsigs)
+      | .mk f args ret =>
+        decidable_of_iff (∃ _ : f < fsigs.length, ⟨args.length, ret⟩ = fsigs[f])
+          ⟨λ ⟨p, q⟩ => ⟨p, q⟩, λ ⟨p, q⟩ => ⟨p, q⟩⟩
 
-  instance instDecidable {fsigs : FuncSigs} : (sc : SpawnCall) -> Decidable (sc.Okay fsigs)
-    | mk f args ret =>
-      decidable_of_iff (∃ _ : f < fsigs.length, ⟨args.length, ret⟩ = fsigs[f])
-        ⟨λ ⟨p, q⟩ => Okay.mk p q,
-         λ | Okay.mk p q => ⟨p, q⟩⟩
+    theorem flt {fsigs} {sc : SpawnCall} : sc.WF fsigs -> sc.f < fsigs.length | mk flt _ => flt
+    theorem sig {fsigs} {sc : SpawnCall} : (wf : sc.WF fsigs) -> ⟨sc.args.length, sc.ret⟩ = fsigs[sc.f]'wf.flt | mk _ sig => sig
+  end WF
   
-  -- instance instDecidableEq : DecidableEq SpawnCall
-  --   | mk f args ret, mk f' args' ret' =>
-  --     decidable_of_iff ((f, args, ret) = (f', args', ret'))
-  --       ⟨congrArg (λ (f, args, ret) => mk f args ret),
-  --        congrArg (λ | mk f args ret => (f, args, ret))⟩
   deriving instance DecidableEq for SpawnCall
 end SpawnCall
 
 namespace SpawnDeque
-  abbrev unpr : SpawnDeque -> List SpawnCall
+  @[simp] abbrev unpr : SpawnDeque -> List SpawnCall
     | ⟨u, _p⟩ => u
-  abbrev prom : SpawnDeque -> SporkSig
+  @[simp] abbrev prom : SpawnDeque -> SporkSig
     | ⟨_u, p⟩ => p
 
   abbrev SpawnOrder (canProm : Bool) (prom : SporkSig) : Prop :=
@@ -261,159 +239,216 @@ namespace SpawnDeque
       | true, _gret, _prom, _so => rfl
   end SpawnOrder
 
-  inductive Okay (fsigs : FuncSigs) (canProm : Bool) : SpawnDeque -> Prop
+  instance : EmptyCollection SpawnDeque := ⟨⟨[], []⟩⟩
+
+  inductive WF (fsigs : FuncSigs) (canProm : Bool) : SpawnDeque -> Prop
     | mk {unpr : List SpawnCall} {prom : SporkSig} :
-         IVec (·.Okay fsigs) unpr ->
+         IVec (·.WF fsigs) unpr ->
          SpawnOrder canProm prom ->
-         (mk unpr prom).Okay fsigs canProm
+         (mk unpr prom).WF fsigs canProm
 
-  namespace Okay
-    abbrev unpr {fsigs canProm} {ρ : SpawnDeque} : ρ.Okay fsigs canProm -> IVec (·.Okay fsigs) ρ.unpr | mk u _p => u
-    abbrev prom {fsigs canProm} {ρ : SpawnDeque} : ρ.Okay fsigs canProm -> SpawnOrder canProm ρ.prom | mk _u p => p
+  namespace WF
+    instance {fsigs canProm} : (ρ : SpawnDeque) -> Decidable (ρ.WF fsigs canProm)
+      | .mk u p => decidable_of_iff
+          (IVec (·.WF fsigs) u ∧ SpawnOrder canProm p)
+          ⟨λ ⟨a, b⟩ => ⟨a, b⟩, λ ⟨a, b⟩ => ⟨a, b⟩⟩
+    
+    theorem unpr {fsigs canProm} {ρ : SpawnDeque} : ρ.WF fsigs canProm -> IVec (·.WF fsigs) ρ.unpr | mk u _p => u
+    theorem prom {fsigs canProm} {ρ : SpawnDeque} : ρ.WF fsigs canProm -> SpawnOrder canProm ρ.prom | mk _u p => p
 
-    theorem castCanProm {fsigs ρ} : {canProm : Bool} -> (canProm' : Bool) -> canProm ≤ canProm' -> Okay fsigs canProm ρ -> Okay fsigs canProm' ρ
+    theorem castCanProm {fsigs ρ} : {canProm : Bool} -> (canProm' : Bool) -> canProm ≤ canProm' -> WF fsigs canProm ρ -> WF fsigs canProm' ρ
       | false, false, _, .mk u p => .mk u p
       | true, true, _, .mk u p => .mk u p
       | false, true, _, .mk u _p => .mk u rfl
 
-    theorem promote {fsigs u p g} (ok : Okay fsigs true ⟨g :: u, p⟩) :
-                    Okay fsigs true ⟨u, g.ret :: p⟩ :=
-      ⟨ok.unpr.tail, rfl⟩
-  end Okay
+    theorem promote {fsigs u p g} (wf : WF fsigs true ⟨g :: u, p⟩) :
+                    WF fsigs true ⟨u, g.ret :: p⟩ :=
+      ⟨wf.unpr.tail, rfl⟩
+
+    theorem empty {fsigs canProm} : SpawnDeque.WF fsigs canProm ∅ :=
+      ⟨.nil, .of_nil⟩
+  end WF
   
-  abbrev sig : SpawnDeque -> SporkSig
+  @[simp] def sig : SpawnDeque -> SporkSig
     | mk u p => List.reverseAux (u.map (·.ret)) p
-  abbrev push : SpawnDeque -> SpawnCall -> SpawnDeque
+  @[simp] def push : SpawnDeque -> SpawnCall -> SpawnDeque
     | ⟨u, p⟩, sc => ⟨u.concat sc, p⟩
-  abbrev pop_prom : SpawnDeque -> SpawnDeque
+  @[simp] def pop_prom : SpawnDeque -> SpawnDeque
     | ⟨sc :: u, p⟩ => ⟨u, sc.ret :: p⟩
     | ⟨[], p⟩ => ⟨[], p⟩
   theorem pushsig (ρ : SpawnDeque) (sc : SpawnCall)
                   : (ρ.push sc).sig = sc.ret :: ρ.sig :=
     by simp
-  instance empty_collection : EmptyCollection SpawnDeque := ⟨⟨[], []⟩⟩
 
-  instance instDecidable {fsigs canProm} : (ρ : SpawnDeque) -> Decidable (ρ.Okay fsigs canProm)
-    | mk u p => decidable_of_iff
-        (IVec (·.Okay fsigs) u ∧ SpawnOrder canProm p)
-        ⟨λ ⟨a, b⟩ => Okay.mk a b, λ | Okay.mk a b => ⟨a, b⟩⟩
-
-  -- instance instDecidableEq : DecidableEq SpawnDeque
-  --   | mk u p, mk u' p' => decidable_of_iff ((u, p) = (u', p'))
-  --     ⟨congrArg (λ (u, p) => mk u p),
-  --      congrArg (λ | mk u p => (u, p))⟩
   deriving instance DecidableEq for SpawnDeque
-
-  theorem empty_okay {fsigs canProm} : SpawnDeque.Okay fsigs canProm ∅ :=
-    ⟨.nil, .of_nil⟩
 end SpawnDeque
 
 namespace StackFrame
-  abbrev f | mk f _ρ _X _c => f
-  abbrev ρ | mk _f ρ _X _c => ρ
-  abbrev X | mk _f _ρ X _c => X
-  abbrev c | mk _f _ρ _X c => c
-  abbrev bsig | mk _f ρ X _c => BlockSig.mk X.length ρ.sig
+  @[simp] abbrev f | mk f _ρ _X _c => f
+  @[simp] abbrev ρ | mk _f ρ _X _c => ρ
+  @[simp] abbrev X | mk _f _ρ X _c => X
+  @[simp] abbrev c | mk _f _ρ _X c => c
+  @[simp] def bsig | mk _f ρ X _c => BlockSig.mk X.length ρ.sig
 
-  inductive Okay (Pr : Program) (curr : Option Nat) (canProm : Bool) : StackFrame -> Prop where
+  inductive WF (P : Program) (curr : Option Nat) (canProm : Bool) :
+               (K : StackFrame) -> Prop where
     | mk {f ρ X c} :
-         (_ : f < Pr.size) ->
-         ρ.Okay Pr.fsigs canProm ->
+         (_ : f < P.size) ->
+         ρ.WF P.fsigs canProm ->
          (if curr.isNone then c.isCode else c.isCont) = true ->
-         c.Okay Pr.fsigs Pr.funs[f].bsigs ⟨X.length, ρ.sig⟩
-                (curr.elim Pr.funs[f].fsig.ret id) ->
-         (mk f ρ X c).Okay Pr curr canProm
+         c.WF P.fsigs P[f].bsigs ⟨X.length, ρ.sig⟩
+                (curr.elim P[f].fsig.ret id) ->
+         (mk f ρ X c).WF P curr canProm
 
-  namespace Okay
-    theorem flt {Pr curr canProm} : {k : StackFrame} -> k.Okay Pr curr canProm -> k.f < Pr.size
-      | .mk _f _ρ _X _c, mk flt _ρₒₖ _cₒₖ _cb => flt
-  end Okay
+  namespace WF
+    instance {P curr canProm} : (k : StackFrame) -> Decidable (k.WF P curr canProm)
+      | .mk f ρ X c =>
+        decidable_of_iff (∃ _ : f < P.size,
+                          ρ.WF P.fsigs canProm ∧
+                          (if curr.isNone then c.isCode else c.isCont) = true ∧
+                          c.WF P.fsigs P[f].bsigs ⟨X.length, ρ.sig⟩
+                            (curr.elim P[f].fsig.ret id))
+          ⟨λ ⟨a, b, c, d⟩ => ⟨a, b, c, d⟩, λ ⟨a, b, c, d⟩ => ⟨a, b, c, d⟩⟩
 
-  abbrev func {Pr curr canProm} (k : StackFrame) (kₒₖ : k.Okay Pr curr canProm) : Func :=
-    Pr.funs[k.f]'kₒₖ.flt
+    theorem flt {P curr canProm} : {k : StackFrame} ->
+                k.WF P curr canProm -> k.f < P.size
+      | .mk _f _ρ _X _c, mk flt _ρwf _cwf _cb => flt
+  end WF
 
-  namespace Okay
-    -- abbrev func {Pr curr canProm} {k : StackFrame} (kₒₖ : k.Okay Pr curr canProm) : Func :=
-    --   k.func kₒₖ
-    -- abbrev ret {Pr curr canProm} {k : StackFrame} (kₒₖ : k.Okay Pr curr canProm) : Nat :=
-    --   kₒₖ.func.fsig.ret
-    theorem ρₒₖ {Pr curr canProm} : {k : StackFrame} -> k.Okay Pr curr canProm -> k.ρ.Okay Pr.fsigs canProm
-      | .mk _f _ρ _X _c, mk _flt ρₒₖ _cₒₖ _cb => ρₒₖ
-    theorem cₒₖ {Pr curr canProm} : {k : StackFrame} -> (kₒₖ : k.Okay Pr curr canProm) ->
-                k.c.Okay Pr.fsigs (k.func kₒₖ).bsigs k.bsig
-                         (curr.elim (k.func kₒₖ).fsig.ret id)
-      | .mk _f _ρ _X _c, mk _flt _ρₒₖ _cb cₒₖ => cₒₖ
-    theorem cₒₖ' {Pr curr canProm} : {k : StackFrame} -> (kₒₖ : k.Okay Pr curr canProm) ->
-                 k.c.Okay Pr.fsigs Pr.funs[k.f]!.bsigs k.bsig
-                          (curr.elim Pr.funs[k.f]!.fsig.ret id)
-      | .mk f _ρ _X _c, mk flt _ρₒₖ _cb cₒₖ =>
-        getElem!_pos Pr.funs f flt ▸ cₒₖ
-    theorem cₒₖ'' {Pr curr canProm} : {k : StackFrame} -> (kₒₖ : k.Okay Pr curr canProm) ->
-                  let flt : k.f < Pr.size := kₒₖ.flt
-                  k.c.Okay Pr.fsigs Pr.funs[k.f].bsigs k.bsig
-                           (curr.elim Pr.funs[k.f].fsig.ret id)
-      | .mk _f _ρ _X _c, mk _flt _ρₒₖ _cb cₒₖ => cₒₖ
-    theorem cb {Pr curr canProm} : {k : StackFrame} -> (kₒₖ : k.Okay Pr curr canProm) ->
+  @[simp] def func {P curr canProm} (k : StackFrame) (kwf : k.WF P curr canProm) : Func :=
+    P[k.f]'kwf.flt
+
+  namespace WF
+
+    theorem ρwf {P curr canProm} : {k : StackFrame} ->
+                k.WF P curr canProm -> k.ρ.WF P.fsigs canProm
+      | .mk _f _ρ _X _c, mk _flt ρwf _cwf _cb => ρwf
+    theorem cwf {P curr canProm} : {k : StackFrame} -> (kwf : k.WF P curr canProm) ->
+                k.c.WF P.fsigs (k.func kwf).bsigs k.bsig
+                         (curr.elim (k.func kwf).fsig.ret id)
+      | .mk _f _ρ _X _c, mk _flt _ρwf _cb cwf => cwf
+    theorem cwf' {P curr canProm} : {k : StackFrame} -> (kwf : k.WF P curr canProm) ->
+                 k.c.WF P.fsigs P[k.f]!.bsigs k.bsig
+                          (curr.elim P[k.f]!.fsig.ret id)
+      | .mk f _ρ _X _c, mk flt _ρwf _cb cwf =>
+        getElem!_pos P f flt ▸ cwf
+    theorem cwf'' {P curr canProm} : {k : StackFrame} -> (kwf : k.WF P curr canProm) ->
+                  let flt : k.f < P.size := kwf.flt
+                  k.c.WF P.fsigs P[k.f].bsigs k.bsig
+                           (curr.elim P[k.f].fsig.ret id)
+      | .mk _f _ρ _X _c, mk _flt _ρwf _cb cwf => cwf
+    theorem cb {P curr canProm} : {k : StackFrame} -> (kwf : k.WF P curr canProm) ->
                (if curr.isNone then k.c.isCode else k.c.isCont) = true
-      | .mk _f _ρ _X _c, mk _flt _ρₒₖ cb _cₒₖ => cb
-    theorem isCode {Pr canProm} : {k : StackFrame} ->
-                   (kₒₖ : k.Okay Pr none canProm) -> k.c.isCode := cb
-    theorem isCont {Pr canProm ret} : {k : StackFrame} ->
-                   (kₒₖ : k.Okay Pr (some ret) canProm) -> k.c.isCont := cb
+      | .mk _f _ρ _X _c, mk _flt _ρwf cb _cwf => cb
+    theorem isCode {P canProm} : {k : StackFrame} ->
+                   (kwf : k.WF P none canProm) -> k.c.isCode := cb
+    theorem isCont {P canProm ret} : {k : StackFrame} ->
+                   (kwf : k.WF P (some ret) canProm) -> k.c.isCont := cb
 
-    theorem castCanProm {Pr curr canProm} : {k : StackFrame} ->
+    theorem castCanProm {P curr canProm} : {k : StackFrame} ->
                         (canProm' : Bool) -> canProm ≤ canProm' ->
-                        (kₒₖ : k.Okay Pr curr canProm) -> k.Okay Pr curr canProm'
-      | .mk _f _ρ _X _c, canProm', l, .mk flt ρₒₖ cₒₖ cb =>
-        .mk flt (ρₒₖ.castCanProm canProm' l) cₒₖ cb
-  end Okay
+                        (kwf : k.WF P curr canProm) -> k.WF P curr canProm'
+      | .mk _f _ρ _X _c, canProm', l, .mk flt ρwf cwf cb =>
+        .mk flt (ρwf.castCanProm canProm' l) cwf cb
 
-  instance instDecidable {Pr curr canProm} : (k : StackFrame) -> Decidable (k.Okay Pr curr canProm)
-    | mk f ρ X c =>
-      decidable_of_iff (∃ _ : f < Pr.size,
-                        ρ.Okay Pr.fsigs canProm ∧
-                        (if curr.isNone then c.isCode else c.isCont) = true ∧
-                        c.Okay Pr.fsigs Pr.funs[f].bsigs ⟨X.length, ρ.sig⟩
-                          (curr.elim Pr.funs[f].fsig.ret id))
-        ⟨λ ⟨a, b, c, d⟩ => Okay.mk a b c d,
-         λ | Okay.mk a b c d => ⟨a, b, c, d⟩⟩
+    theorem entry
+        {P} (Pwf : P.WF) {f canProm} {X : List Val}
+        (p : f < P.size)
+        (sigwf : P[f].fsig.arity = X.length) :
+        WF P none canProm ⟨f, ∅, X, .codeEntry P f⟩ :=
+      let fwf := Pwf.1.get ⟨f, p⟩
+      let c' : Code.WF P.fsigs P[f].bsigs P[f].fsig.ret
+                ⟨X.length, []⟩ P[f]!.blocks.head!.code :=
+        sigwf ▸
+        Eq.symm (getElem!_pos P f p) ▸
+        fwf.2.headeq ▸
+        fwf.2.head!eq ▸
+        (fwf.1.head fwf.2.nonnil).1
+      ⟨p, SpawnDeque.WF.empty, rfl, .code c'⟩
 
-  -- instance instDecidableEq : DecidableEq StackFrame
-  --   | mk f ρ X c, mk f' ρ' X' c' =>
-  --     decidable_of_iff ((f, ρ, X, c) = (f', ρ', X', c'))
-  --       ⟨congrArg (λ (a, b, c, d) => mk a b c d),
-  --        congrArg (λ | mk a b c d => (a, b, c, d))⟩
+    theorem goto_rets
+        {P} (Pwf : P.WF) {f canProm ρ} {X Y : ValMap} {bnext} {y : List Var}
+        (p : f < P.size)
+        (ρwf : ρ.WF P.fsigs canProm)
+        (bnext_wf : bnext.WFRets P[f].bsigs ⟨X.length, ρ.sig⟩ y.length)
+        (y_wf : IVec (·.WF Y.length) y) :
+        StackFrame.WF P none canProm
+          ⟨f, ρ, X[bnext.args]! ++ Y[y]!, .codeOf P f bnext⟩ :=
+      let ⟨bwf, sigwf, x_wf⟩ := bnext_wf
+      let bwf' : bnext.b < P[f].size :=
+        by simp; exact (List.length_map Block.bsig ▸ bwf)
+      let xlen : bnext.args.length = X[bnext.args].length :=
+        x_wf.map_length (λ x xwf => X[x])
+      let ylen : y.length = Y[y].length :=
+        y_wf.map_length (λ y ywf => Y[y])
+      let code_wf : P[f]![bnext.b]!.code.WF
+                      P.fsigs P[f].bsigs P[f].fsig.ret
+                      ⟨(X[bnext.args]! ++ Y[y]!).length, ρ.sig⟩ := by
+        rw[codeOfGetElem p bwf',
+           argsOfGetElem x_wf,
+           argsOfGetElem y_wf,
+           List.length_append,
+           ← xlen, ← ylen]
+        simp at sigwf
+        simp
+        rw[← sigwf];
+        exact ((Pwf.1.get ⟨f, p⟩).1.get ⟨bnext.b, bwf'⟩).1
+      ⟨p, ρwf, rfl, .code code_wf⟩
+  
+    theorem goto
+        {P} (Pwf : P.WF) {f canProm ρ} {X : ValMap} {bnext}
+        (p : f < P.size)
+        (ρwf : ρ.WF P.fsigs canProm)
+        (bnext_wf : bnext.WF P[f].bsigs ⟨X.length, ρ.sig⟩) :
+        StackFrame.WF P none canProm ⟨f, ρ, X[bnext.args]!, .codeOf P f bnext⟩ :=
+      List.append_nil X[bnext.args]! ▸
+      goto_rets Pwf (Y := []) (y := []) p ρwf bnext_wf.cast0 .nil
+  
+    theorem goto_entry
+        {P} (Pwf : P.WF) {f canProm} {X : ValMap} {x : List Var}
+        (p : f < P.size)
+        (xwf : IVec (·.WF X.length) x)
+        (sigwf : P[f].fsig.arity = x.length) :
+        StackFrame.WF P none canProm ⟨f, ∅, X[x]!, .codeEntry P f⟩ :=
+      entry Pwf p (argsOfGetElem xwf ▸
+                    xwf.map_length (λ x xwf => X[x]) ▸
+                    sigwf)
+  
+  end WF
+
   deriving instance DecidableEq for StackFrame
 end StackFrame
 
 namespace CallStack
   notation (name := callstackcons) t " ⬝ " h:arg => cons t h
 
-  abbrev appendh : CallStack -> CallStack -> CallStack
+  @[simp] def append : CallStack -> CallStack -> CallStack
     | K, nil => K
-    | K, K' ⬝ k => (appendh K K') ⬝ k
+    | K, K' ⬝ k => (CallStack.append K K') ⬝ k
 
-  instance instAppend : Append CallStack where
-    append := appendh
-  instance instSingleton : Singleton StackFrame CallStack where
+  instance : Append CallStack where
+    append := CallStack.append
+  instance : Singleton StackFrame CallStack where
     singleton k := nil ⬝ k
-  instance instEmptyCollection : EmptyCollection CallStack where
+  instance : EmptyCollection CallStack where
     emptyCollection := nil
+  instance : Inhabited CallStack where
+    default := nil
 
-  abbrev prom : CallStack -> SporkSig
+  @[simp] def prom : CallStack -> SporkSig
     | nil => []
     | K ⬝ k => k.ρ.prom ++ prom K
-  abbrev unpr : CallStack -> List SpawnCall
+  @[simp] def unpr : CallStack -> List SpawnCall
     | nil => []
     | K ⬝ k => unpr K ++ k.ρ.unpr
-  abbrev allPromoted (K : CallStack) : Bool := K.unpr = []
-  abbrev allPromoted_imp_nil {K} (p : allPromoted K) : K.unpr = [] := by simp_all
-  abbrev nil_imp_allPromoted {K} (p : unpr K = []) : K.allPromoted := by simp_all
-  abbrev firstFrame : (K : CallStack) -> K ≠ nil -> StackFrame
+  @[simp] abbrev allPromoted (K : CallStack) : Bool := K.unpr = []
+  @[simp] def firstFrame : (K : CallStack) -> K ≠ nil -> StackFrame
     | nil ⬝ k, p => k
     | K  ⬝ k ⬝ _k', p => firstFrame (K ⬝ k) (by simp)
 
-  @[simp] theorem append_cons : {K K' : CallStack} -> {k : StackFrame} -> K ++ (K' ⬝ k) = (K ++ K') ⬝ k
+  @[simp] theorem append_eq {as bs} : append as bs = as ++ bs := rfl
+  @[simp] theorem append_cons : {K K' : CallStack} -> {k : StackFrame} ->
+                                K ++ (K' ⬝ k) = (K ++ K') ⬝ k
     | _K, nil, _k => rfl
     | _K, _K' ⬝ _k', k => congrArg (· ⬝ k) append_cons
   @[simp] theorem append_nil : {K : CallStack} -> K ++ nil = K := rfl
@@ -424,322 +459,313 @@ namespace CallStack
     | _K, _K', nil => rfl
     | _K, _K', _K'' ⬝ k =>
       append_cons ▸ append_cons ▸ congrArg (· ⬝ k) append_assoc
-  theorem append_unpr : {K K' : CallStack} -> (K ++ K').unpr = K.unpr ++ K'.unpr
+  @[simp] theorem append_unpr : {K K' : CallStack} -> (K ++ K').unpr = K.unpr ++ K'.unpr
     | K, nil => by simp
-    | K, K' ⬝ k => by simp[unpr]; rw[← List.append_assoc, ← append_unpr]; rfl
-  theorem append_prom : {K K' : CallStack} -> (K ++ K').prom = K'.prom ++ K.prom
+    | K, K' ⬝ k =>
+      append_cons ▸
+      List.append_assoc K.unpr K'.unpr k.ρ.unpr ▸
+      @append_unpr K K' ▸
+      rfl
+  --@[simp] theorem append_unpr_ : {K K' : CallStack} -> (K.append K').unpr = K.unpr ++ K'.unpr := append_unpr
+  @[simp] theorem append_prom : {K K' : CallStack} -> (K ++ K').prom = K'.prom ++ K.prom
     | K, nil => by simp
     | K, K' ⬝ k => by simp; exact append_prom
-  -- theorem prom_nil_of_cons {K k} : (K ⬝ k).prom = [] -> k.ρ.prom = [] ∧ K.prom = [] :=
-  --   List.append_eq_nil_iff.mp
 
-  abbrev head : (K : CallStack) -> K ≠ nil -> StackFrame
+  theorem allPromoted_iff_nil {K} : allPromoted K <-> K.unpr = [] :=
+    by simp
+  theorem allPromoted_cons {K k} : allPromoted (K ⬝ k) <->
+                                   allPromoted K ∧ k.ρ.unpr = [] :=
+    by simp
+  theorem allPromoted_append {K K'} : allPromoted (K ++ K') <->
+                                      K.allPromoted ∧ K'.allPromoted :=
+    by simp
+
+  @[simp] def head : (K : CallStack) -> K ≠ nil -> StackFrame
     | _K ⬝ k, _ => k
-  abbrev tail : CallStack -> CallStack
+  @[simp] def tail : CallStack -> CallStack
     | K ⬝ _k => K
     | nil => nil
 
-  abbrev retjoin (Pr : Program) : CallStack -> Nat
+  @[simp] def retjoin (P : Program) : CallStack -> Nat
     | nil => default
-    | nil ⬝ ⟨f, _, _, _⟩ => Pr.funs[f]!.fsig.ret
-    | K ⬝ _k => K.retjoin Pr
+    | nil ⬝ ⟨f, _, _, _⟩ => P[f]!.fsig.ret
+    | K ⬝ _k => K.retjoin P
 
-  @[simp] theorem retjoin_first {Pr : Program} : {k : StackFrame} -> {K : CallStack} -> ({k} ++ K).retjoin Pr = Pr.funs[k.f]!.fsig.ret
-    | k, .nil => rfl
-    | k, .nil ⬝ k' => rfl
-    | k, K ⬝ k' ⬝ k'' => by
-        simp only[retjoin]
-        exact retjoin_first (K := K ⬝ k')
+  @[simp] theorem retjoin_first {P : Program} : {k : StackFrame} -> {K : CallStack} ->
+                                ({k} ++ K).retjoin P = P[k.f]!.fsig.ret
+    | _k, .nil => rfl
+    | _k, .nil ⬝ _k' => rfl
+    | _k, K ⬝ k' ⬝ _k'' => retjoin_first (K := K ⬝ k')
 
-  inductive Okay (Pr : Program) : (get : Option Nat) -> CallStack -> Prop where
-    | nil {gets} : nil.Okay Pr (some gets)
+  /--
+  (Potentially partial) call stack.
+  When `get` is omitted (`none`), this must be a full call
+  stack, where the current frame has `code` rather than `cont`
+  When `get` is `some n`, it is a partial call stack awaiting
+  a return of `n` args from the following stack frame
+  -/
+  inductive WF (P : Program) : (get : Option Nat := none) -> CallStack -> Prop where
+    | nil {gets} : nil.WF P (some gets)
     | cons {K k gets} :
-           (kₒₖ : k.Okay Pr gets K.allPromoted) ->
-           K.Okay Pr (k.func kₒₖ).fsig.ret ->
-           (K ⬝ k).Okay Pr gets
+           (kwf : k.WF P gets K.allPromoted) ->
+           K.WF P (k.func kwf).fsig.ret ->
+           (K ⬝ k).WF P gets
 
-  namespace Okay
-    notation (name := callstackokaycons) t " ⬝ₒₖ " h:arg => Okay.cons h t
-    theorem nonnil {Pr} {K : CallStack} (Kₒₖ : K.Okay Pr none) : K ≠ CallStack.nil :=
-      by cases Kₒₖ; simp
-    theorem head' {Pr gets} :
+  namespace WF
+    notation (name := callstackwfcons) t " ⬝wf " h:arg => WF.cons h t
+
+    instance instDecidable {P} : {gets : Option Nat} -> (K : CallStack) ->
+                           Decidable (K.WF P gets)
+      | some gets, .nil => isTrue WF.nil
+      | none, .nil => isFalse (by cases ·)
+      | gets, K ⬝ k =>
+        dite (k.WF P gets K.allPromoted)
+          (λ kwf => let Kwfdec : Decidable (K.WF P (some (k.func kwf).fsig.ret)) :=
+                      instDecidable K
+                    decidable_of_iff (K.WF P (some (k.func kwf).fsig.ret))
+                      ⟨cons kwf, λ | cons _kwf' Kwf => Kwf⟩)
+          (isFalse ∘ λ | kₙwf, cons kwf _Kwf => kₙwf kwf)
+
+    theorem nonnil {P} {K : CallStack} (Kwf : K.WF P none) : K ≠ CallStack.nil :=
+      by cases Kwf <;> simp
+    theorem head' {P gets} :
                   {K : CallStack} ->
                   (nn : K ≠ CallStack.nil) ->
-                  K.Okay Pr gets ->
-                  (K.head nn).Okay Pr gets K.tail.allPromoted
-      | _K ⬝ _k, _nn, _Kₒₖ ⬝ₒₖ kₒₖ => kₒₖ
-    theorem tail' {Pr gets} :
+                  K.WF P gets ->
+                  (K.head nn).WF P gets K.tail.allPromoted
+      | _K ⬝ _k, _nn, _Kwf ⬝wf kwf => kwf
+    theorem tail' {P gets} :
                   {K : CallStack} ->
                   (nn : K ≠ CallStack.nil) ->
-                  (Kₒₖ : K.Okay Pr gets) ->
-                  K.tail.Okay Pr (some (Pr.funs[(K.head nn).f]'(Kₒₖ.head' nn).flt).fsig.ret)
-      | _K ⬝ _k, _nn, Kₒₖ ⬝ₒₖ _kₒₖ => Kₒₖ
+                  (Kwf : K.WF P gets) ->
+                  K.tail.WF P (some (P[(K.head nn).f]'(Kwf.head' nn).flt).fsig.ret)
+      | _K ⬝ _k, _nn, Kwf ⬝wf _kwf => Kwf
 
-    theorem head {Pr gets K k} (Kₒₖ : (K ⬝ k).Okay Pr gets) :
-                 k.Okay Pr gets K.allPromoted :=
-      head' (by simp) Kₒₖ
+    theorem head {P gets K k} (Kwf : (K ⬝ k).WF P gets) :
+                 k.WF P gets K.allPromoted :=
+      head' (by simp) Kwf
 
-    theorem tail {Pr gets K k} (Kₒₖ : (K ⬝ k).Okay Pr gets) :
-                  K.Okay Pr (some (Pr.funs[k.f]'Kₒₖ.head.flt).fsig.ret) :=
-      tail' (by simp) Kₒₖ
-  end Okay
-
-  instance instDecidable {Pr} : {gets : Option Nat} -> (K : CallStack) -> Decidable (K.Okay Pr gets)
-    | some gets, nil => isTrue Okay.nil
-    | none, nil => isFalse (by cases ·)
-    | gets, K ⬝ k =>
-      dite (k.Okay Pr gets K.allPromoted)
-        (λ kₒₖ => let Kₒₖdec : Decidable (K.Okay Pr (some (k.func kₒₖ).fsig.ret)) := instDecidable K
-                  decidable_of_iff (K.Okay Pr (some (k.func kₒₖ).fsig.ret))
-                    ⟨Okay.cons kₒₖ, λ | Okay.cons _kₒₖ' Kₒₖ => Kₒₖ⟩)
-        (isFalse ∘ λ | kₙₒₖ, .cons kₒₖ _Kₒₖ => kₙₒₖ kₒₖ)
+    theorem tail {P gets K k} (Kwf : (K ⬝ k).WF P gets) :
+                  K.WF P (some (P[k.f]'Kwf.head.flt).fsig.ret) :=
+      tail' (by simp) Kwf
+  end WF
 
   deriving instance DecidableEq for CallStack
-
-  abbrev retjoin?! {Pr get} : (K : CallStack) -> K.Okay Pr get -> Option Nat
-    | .nil, _ok => none
-    | .nil ⬝ k, ok => some (k.func ok.head).fsig.ret
-    | K ⬝ _k, ok => K.retjoin?! ok.tail
   
-  theorem retjoin_eq_retjoin?! {Pr get} : {K : CallStack} -> (ok : K.Okay Pr get) ->
-          (if K = .nil then none else some (K.retjoin Pr)) = K.retjoin?! ok
-    | .nil, ok =>
+  @[simp] def retjoin?! {P get} : (K : CallStack) -> K.WF P get -> Option Nat
+    | .nil, _wf => none
+    | .nil ⬝ k, wf => some (k.func wf.head).fsig.ret
+    | K ⬝ _k, wf => K.retjoin?! wf.tail
+  
+  theorem retjoin_eq_retjoin?! {P get} : {K : CallStack} -> (wf : K.WF P get) ->
+          (if K = .nil then none else some (K.retjoin P)) = K.retjoin?! wf
+    | .nil, _wf =>
       rfl
-    | .nil ⬝ k, (_ ⬝ₒₖ kok) =>
-      by simp[retjoin, getElem!_pos Pr.funs k.f kok.flt]
-    | K ⬝ k ⬝ k', ok =>
-      retjoin_eq_retjoin?! (K := K ⬝ k) ok.tail
+    | .nil ⬝ k, (_ ⬝wf kwf) =>
+      congrArg (α := Func) (λ x => some x.fsig.ret) (getElem!_pos P k.f kwf.flt)
+    | K ⬝ k ⬝ _k', wf =>
+      retjoin_eq_retjoin?! (K := K ⬝ k) wf.tail
 
-  namespace Okay
-
-    theorem append {Pr} : {K K' : CallStack} -> {gets : Option Nat} -> K.Okay Pr (some (K'.retjoin Pr)) -> K'.Okay Pr gets -> (gets.isNone ∨ K' ≠ .nil) -> K.allPromoted -> (K ++ K').Okay Pr gets
-      | K, .nil ⬝ k, gets, Kok, K'ok@(.nil ⬝ₒₖ kok), _, kprom =>
+  namespace WF
+    theorem append {P} : {K K' : CallStack} -> {gets : Option Nat} ->
+                   K.WF P (some (K'.retjoin P)) -> K'.WF P gets ->
+                   (gets.isNone ∨ K' ≠ .nil) -> K.allPromoted -> (K ++ K').WF P gets
+      | K, .nil ⬝ k, gets, Kwf, K'wf@(.nil ⬝wf kwf), _, kprom =>
         by simp; exact
-          (Option.some_inj.mp (retjoin_eq_retjoin?! K'ok) ▸ Kok) ⬝ₒₖ (kprom ▸ kok)
-      | K, K' ⬝ k' ⬝ k, gets, Kok, K'ok ⬝ₒₖ kok, p, kprom =>
-        let kprom' : K.unpr = [] := by simp_all[kprom]
+          (Option.some_inj.mp (retjoin_eq_retjoin?! K'wf) ▸ Kwf) ⬝wf (kprom ▸ kwf)
+      | K, K' ⬝ k' ⬝ k, gets, Kwf, K'wf ⬝wf kwf, p, kprom =>
+        let kprom' := allPromoted_iff_nil.mp kprom
         let kp : (K' ⬝ k').unpr = (K ++ (K' ⬝ k')).unpr :=
-          by simp[append_unpr, kprom']
-        (append Kok K'ok (Or.inr (by simp)) kprom) ⬝ₒₖ
-          (by simp only[allPromoted, kp.symm]; exact kok)
+          by simp; rw[kprom']
+        (append Kwf K'wf (Or.inr (by simp)) kprom) ⬝wf
+          (by simp at kwf; simp; rw[kprom']; exact kwf)
 
-    theorem unappend {Pr} : {get : Option Nat} -> {K K' : CallStack} -> (K ++ K').Okay Pr get -> (K' ≠ .nil) ->
-                     K.allPromoted -> K.Okay Pr (some (K'.retjoin Pr)) ∧ K'.Okay Pr get
-      | get, K, .nil ⬝ k, ok, _, kprom =>
-        let ok' : (K ⬝ k).Okay Pr get :=
-          by rw[@append_cons K .nil k] at ok; exact ok
-        let k_ok : k.Okay Pr get true :=
-          kprom ▸ ok'.head
-        ⟨by simp[retjoin]
-            rw[getElem?_pos Pr.funs k.f k_ok.flt]
-            exact ok'.tail,
-         .nil ⬝ₒₖ k_ok⟩
-      | get, K, (K' ⬝ k') ⬝ k, ok, _, kprom =>
-        let ⟨Kok, K'ok⟩ := unappend ok.tail (by simp) kprom
-        let kprom' : K.unpr = [] := by simp_all[kprom]
+    theorem unappend {P} : {get : Option Nat} -> {K K' : CallStack} ->
+                     (K ++ K').WF P get -> (K' ≠ .nil) -> K.allPromoted ->
+                     K.WF P (some (K'.retjoin P)) ∧ K'.WF P get
+      | get, K, .nil ⬝ k, wf, _, kprom =>
+        let wf' : (K ⬝ k).WF P get :=
+          by rw[@append_cons K .nil k] at wf; exact wf
+        let k_wf : k.WF P get true :=
+          kprom ▸ wf'.head
+        ⟨by simp only[retjoin]
+            rw[getElem!_pos P k.f k_wf.flt]
+            exact wf'.tail,
+         .nil ⬝wf k_wf⟩
+      | get, K, (K' ⬝ k') ⬝ k, wf, _, kprom =>
+        let ⟨Kwf, K'wf⟩ := unappend wf.tail (by simp) kprom
+        let kprom' := allPromoted_iff_nil.mp kprom
         let kp : [] ++ (K' ⬝ k').unpr = K.unpr ++ (K' ⬝ k').unpr :=
           kprom'.symm ▸ rfl
-        let k'ok : k.Okay Pr get (K' ⬝ k').allPromoted := by
-          show k.Okay Pr get ((K' ⬝ k').unpr = [])
+        let k'wf : k.WF P get (K' ⬝ k').allPromoted := by
+          show k.WF P get ((K' ⬝ k').unpr = [])
           rw[← List.nil_append (K' ⬝ k').unpr, kp, ← append_unpr]
-          exact ok.head
-        ⟨Kok, K'ok ⬝ₒₖ k'ok⟩
-  end Okay
+          exact wf.head
+        ⟨Kwf, K'wf ⬝wf k'wf⟩
+  end WF
 end CallStack
 
-namespace ThreadPool
-  instance instAppend : Append ThreadPool where
-    append := cat
-  instance instSingleton : Singleton CallStack ThreadPool where
-    singleton := ThreadPool.leaf
-  instance instInsert : Insert CallStack ThreadPool where
+namespace ThreadTree
+  instance : Append ThreadTree where
+    append := node
+  instance : Singleton CallStack ThreadTree where
+    singleton := thread
+  instance : Insert CallStack ThreadTree where
     insert s p := {s} ++ p
+  instance : Inhabited ThreadTree where
+    default := thread default
 
-  abbrev retjoin (Pr : Program) : ThreadPool -> Nat
-    | leaf K => K.retjoin Pr
-    | cat P _P' => P.retjoin Pr
+  @[simp] def retjoin (P : Program) : ThreadTree -> Nat
+    | thread K => K.retjoin P
+    | node Rp _Rc => Rp.retjoin P
 
-  abbrev prom : ThreadPool -> SporkSig
-    | leaf K => K.prom
-    | cat P _P' => P.prom.tail
+  @[simp] def prom : ThreadTree -> SporkSig
+    | thread K => K.prom
+    | node Rp _Rc => Rp.prom.tail
 
-  inductive Okay (Pr : Program) : (ρ : SporkSig) -> ThreadPool -> Prop where
-    | leaf {K} :
-           (Kₒₖ : K.Okay Pr none) ->
-           (leaf K).Okay Pr K.prom
-    | cat {P P' ρ} :
-          (Pₒₖ : P.Okay Pr (P'.retjoin Pr :: ρ)) ->
-          (P'ₒₖ : P'.Okay Pr []) ->
-          (cat P P').Okay Pr ρ
+  @[simp] def spawn (P : Program) (f : FuncIdx) (args : List Val) : ThreadTree :=
+    thread (.nil ⬝ ⟨f, ∅, args, .codeEntry P f⟩)
 
-  namespace Okay
-    abbrev get {Pr K ρ} : (ThreadPool.leaf K).Okay Pr ρ -> K.Okay Pr none
-      | leaf Kₒₖ => Kₒₖ
-    abbrev right {Pr P P' ρ} : (ThreadPool.cat P P').Okay Pr ρ -> P'.Okay Pr []
-      | cat _Pₒₖ P'ₒₖ => P'ₒₖ
-    abbrev left {Pr P P' ρ} : (ok : (ThreadPool.cat P P').Okay Pr ρ) -> P.Okay Pr (P'.retjoin Pr :: ρ)
-      | cat Pₒₖ _P'ₒₖ => Pₒₖ
-    
-    theorem same_prom {Pr} : {P : ThreadPool} -> {ρ : SporkSig} ->
-                      P.Okay Pr ρ -> P.prom = ρ
-      | .cat P₁ P₂, ρ, .cat P₁ₒₖ P₂ₒₖ =>
-        by simp[ThreadPool.prom, same_prom (ρ := P₂.retjoin Pr :: ρ) P₁ₒₖ]
-      | .leaf K, .(K.prom), .leaf Kₒₖ => rfl
-  end Okay
+  @[simp] def init (P : Program) : ThreadTree :=
+    let main := 0 -- first function in program is main()
+    spawn P main []
 
-  -- TODO: generalize for child threads not starting from main
-  abbrev init : ThreadPool := {{StackFrame.mk 0 ∅ ∅ (.cont (Cont.mk 0 []))}}
-  abbrev child (f : FuncIdx) (args : List Val) : ThreadPool :=
-    let vs := (List.range args.length).map Var.mk
-    {{StackFrame.mk f ∅ args (.cont (Cont.mk 0 vs))}}
+  deriving instance DecidableEq for ThreadTree
 
-  instance instDecidable {Pr} : {ρ : SporkSig} -> (P : ThreadPool) -> Decidable (P.Okay Pr ρ)
-    | ρ, leaf K => decidable_of_iff (ρ = K.prom ∧ K.Okay Pr none)
-        ⟨λ ⟨p, Kₒₖ⟩ => p ▸ Okay.leaf Kₒₖ,
-         λ | Okay.leaf Kₒₖ => ⟨rfl, Kₒₖ⟩⟩
-    | ρ, cat P P' =>
-      let _ : Decidable (P.Okay Pr (P'.retjoin Pr :: ρ)) := instDecidable P
-      let _ : Decidable (P'.Okay Pr []) := instDecidable P'
-      decidable_of_iff (P.Okay Pr (P'.retjoin Pr :: ρ) ∧ P'.Okay Pr [])
-        ⟨λ ⟨Pₒₖ, P'ₒₖ⟩ => Okay.cat Pₒₖ P'ₒₖ,
-         λ | Okay.cat Pₒₖ P'ₒₖ => ⟨Pₒₖ, P'ₒₖ⟩⟩
+  inductive WF (P : Program) : ThreadTree -> Prop where
+    | thread {K} :
+           (Kwf : K.WF P none) ->
+           (thread K).WF P
+    | node {Rp Rc} :
+          (Rpwf : Rp.WF P) ->
+          (Rcwf : Rc.WF P) ->
+          (Rp.prom.head? = some (Rc.retjoin P)) ->
+          (Rc.prom = []) ->
+          (node Rp Rc).WF P
 
-  deriving instance DecidableEq for ThreadPool
+  namespace WF
+    theorem get {P K} : (ThreadTree.thread K).WF P -> K.WF P
+      | thread Kwf => Kwf
+    theorem child {P Rp Rc} : (ThreadTree.node Rp Rc).WF P -> Rc.WF P
+      | node _Rpwf Rcwf _Rpprom _Rcprom => Rcwf
+    theorem parent {P Rp Rc} : (ThreadTree.node Rp Rc).WF P -> Rp.WF P
+      | node Rpwf _Rcwf _Rprom _Rcprom => Rpwf
+    theorem parent_prom {P Rp Rc} : (ThreadTree.node Rp Rc).WF P ->
+                                 Rp.prom.head? = some (Rc.retjoin P)
+      | node _Rpwf _Rcwf Rpprom _Rcprom => Rpprom
+    theorem child_prom {P Rp Rc} : (ThreadTree.node Rp Rc).WF P -> Rc.prom = []
+      | node _Rpwf _Rcwf _Rpprom Rcprom => Rcprom
+  end WF
 
+  namespace WF
+    instance instDecidable {P} : (R : ThreadTree) -> Decidable (R.WF P)
+      | .thread K => decidable_of_iff (K.WF P none)
+          ⟨thread, λ | thread Kwf => Kwf⟩
+      | .node Rp Rc =>
+        let _ : Decidable (Rp.WF P) := instDecidable Rp
+        let _ : Decidable (Rc.WF P) := instDecidable Rc
+        decidable_of_iff (Rp.WF P ∧
+                          Rc.WF P ∧
+                          Rp.prom.head? = some (Rc.retjoin P) ∧
+                          Rc.prom = [])
+          ⟨λ ⟨Rwf, Rcwf, Rp, Rcp⟩ => node Rwf Rcwf Rp Rcp,
+           λ | node Rwf Rcwf Rp Rcp => ⟨Rwf, Rcwf, Rp, Rcp⟩⟩
 
-  inductive Okay' (Pr : Program) : ThreadPool -> Prop where
-    | leaf {K} :
-           (Kₒₖ : K.Okay Pr none) ->
-           (leaf K).Okay' Pr
-    | cat {P P'} :
-          (Pₒₖ : P.Okay' Pr) ->
-          (P'ₒₖ : P'.Okay' Pr) ->
-          (P.prom.head? = some (P'.retjoin Pr)) ->
-          (P'.prom = []) ->
-          (cat P P').Okay' Pr
+    theorem spawn {P f args ret} (Pwf : P.WF) (fwf : SpawnCall.WF P.fsigs (.mk f args ret)) :
+                  (spawn P f args).WF P := by
+      apply thread
+      apply (.nil ⬝wf ·)
+      exact StackFrame.WF.entry Pwf
+              (by simp; rw[← List.length_map]; exact fwf.flt)
+              (List.getElem_map (α := Func) (·.fsig) ▸
+               (congrArg (α := FuncSig) (·.arity) fwf.sig).symm)
 
-  namespace Okay
-    theorem to_okay' {Pr : Program} : {P : ThreadPool} -> {ρ : SporkSig} ->
-                     P.Okay Pr ρ -> P.Okay' Pr
-      | .leaf K, .(K.prom), .leaf Kₒₖ =>
-        .leaf Kₒₖ
-      | .cat _P _P', _ρ, .cat Pₒₖ P'ₒₖ =>
-        .cat Pₒₖ.to_okay' P'ₒₖ.to_okay'
-          (Pₒₖ.same_prom ▸ rfl) P'ₒₖ.same_prom
-  end Okay
+    theorem init {P} (Pwf : P.WF) : (ThreadTree.init P).WF P :=
+      spawn (ret := 1) Pwf
+        (.mk Pwf.main_lt
+             (Pwf.head.get0eq ▸ (List.getElem_map (l := P.funs) (·.fsig)).symm))
+  end WF
 
-  namespace Okay'
-    theorem to_okay {Pr : Program} : {P : ThreadPool} ->
-                     P.Okay' Pr -> P.Okay Pr P.prom
-      | .leaf K, .leaf Kₒₖ =>
-        .leaf Kₒₖ
-      | .cat P P', .cat Pₒₖ P'ₒₖ Pprom P'prom =>
-        match x : P.prom with
-          | Ppromh :: Ppromt =>
-            let x'' : Ppromh = retjoin Pr P' :=
-              congrArg (λ | some h => h | none => Ppromh) (x ▸ Pprom)
-            by simp![x]
-               exact .cat (ρ := Ppromt) (x'' ▸ x ▸ Pₒₖ.to_okay) (P'prom ▸ P'ₒₖ.to_okay)
-          | [] => let y := x ▸ Pprom
-                  by contradiction
-  end Okay'
-
-  theorem okay_iff_okay' {Pr : Program} {P : ThreadPool} : P.Okay Pr P.prom <-> P.Okay' Pr :=
-    ⟨Okay.to_okay', Okay'.to_okay⟩
-
-end ThreadPool
+end ThreadTree
 
 
-@[inline] abbrev codeOf (Pr : Program) (f : FuncIdx) (b : Cont) : StackFrameCode :=
-  .code Pr.funs[f]!.blocks[b.b]!.code
-@[inline] abbrev codeEntry (Pr : Program) (f : FuncIdx) : StackFrameCode :=
-  .code Pr.funs[f]!.blocks.head!.code
+inductive Step (P : Program) : (R R' : ThreadTree) -> Type where
+  | congr_parent {Rp Rp' Rc} :
+    Step P Rp Rp' ->
+    Step P (Rp.node Rc) (Rp'.node Rc)
 
-inductive Step (Pr : Program) : (P P' : ThreadPool) -> Type where
-  | stepₗ {P P' P₂} :
-    Step Pr P P' ->
-    Step Pr (.cat P P₂) (.cat P' P₂)
-
-  | stepᵣ {P₁ P P'} :
-    Step Pr P P' ->
-    Step Pr (.cat P₁ P) (.cat P₁ P')
+  | congr_child {Rp Rc Rc'} :
+    Step P Rc Rc' ->
+    Step P (.node Rp Rc) (.node Rp Rc')
   
   | stmt {f K ρ X e v c} :
     X ⊢ₑₓₚᵣ e ⇓ v ->
-    Step Pr {K ⬝ ⟨f, ρ, X, .code (.stmt e c)⟩}
+    Step P {K ⬝ ⟨f, ρ, X, .code (.stmt e c)⟩}
             {K ⬝ ⟨f, ρ, X.concat v, .code c⟩}
 
   | goto {f K ρ X bnext} :
-    Step Pr {K ⬝ ⟨f, ρ, X, .code (.trfr (.goto bnext))⟩}
-            {K ⬝ ⟨f, ρ, X[bnext.args]!, codeOf Pr f bnext⟩}
+    Step P {K ⬝ ⟨f, ρ, X, .code (.goto bnext)⟩}
+            {K ⬝ ⟨f, ρ, X[bnext.args]!, .codeOf P f bnext⟩}
 
   | ite_true {f K ρ X cond bthen belse n} :
     X ⊢ₐₜₒₘ cond ⇓ n ->
     n ≠ 0 ->
-    Step Pr {K ⬝ ⟨f, ρ, X, .code (.trfr (.ite cond bthen belse))⟩}
-            {K ⬝ ⟨f, ρ, X[bthen.args]!, codeOf Pr f bthen⟩}
+    Step P {K ⬝ ⟨f, ρ, X, .code (.ite cond bthen belse)⟩}
+            {K ⬝ ⟨f, ρ, X[bthen.args]!, .codeOf P f bthen⟩}
 
   | ite_false {f K ρ X cond bthen belse} :
     X ⊢ₐₜₒₘ cond ⇓ 0 ->
-    Step Pr {K ⬝ ⟨f, ρ, X, .code (.trfr (.ite cond bthen belse))⟩}
-            {K ⬝ ⟨f, ρ, X[belse.args]!, codeOf Pr f belse⟩}
+    Step P {K ⬝ ⟨f, ρ, X, .code (.ite cond bthen belse)⟩}
+            {K ⬝ ⟨f, ρ, X[belse.args]!, .codeOf P f belse⟩}
 
   | call {f g K ρ X x bret} :
-    Step Pr {K ⬝ ⟨f, ρ, X, .code (.trfr (.call g x bret))⟩}
-            {K ⬝ ⟨f, ρ, X, .cont bret⟩ ⬝ ⟨g, {}, X[x]!, codeEntry Pr g⟩}
+    Step P {K ⬝ ⟨f, ρ, X, .code (.call g x bret)⟩}
+            {K ⬝ ⟨f, ρ, X, .cont bret⟩ ⬝ ⟨g, {}, X[x]!, .codeEntry P g⟩}
 
   | retn {f g K ρ X Y y bret} :
-    Step Pr {K ⬝ ⟨f, ρ, X, .cont bret⟩ ⬝ ⟨g, {}, Y, .code (.trfr (.retn y))⟩}
-            {K ⬝ ⟨f, ρ, X[bret.args]! ++ Y[y]!, codeOf Pr f bret⟩}
+    Step P {K ⬝ ⟨f, ρ, X, .cont bret⟩ ⬝ ⟨g, {}, Y, .code (.retn y)⟩}
+            {K ⬝ ⟨f, ρ, X[bret.args]! ++ Y[y]!, .codeOf P f bret⟩}
 
   | spork {f K ρ X g g_args bbody} :
-    Step Pr {K ⬝ ⟨f, ρ, X, .code (.trfr (.spork bbody g g_args))⟩}
-            {K ⬝ ⟨f, ρ.push ⟨g, X[g_args]!, Pr.funs[g]!.fsig.ret⟩, X[bbody.args]!, codeOf Pr f bbody⟩}
+    Step P {K ⬝ ⟨f, ρ, X, .code (.spork bbody g g_args)⟩}
+            {K ⬝ ⟨f, ρ.push ⟨g, X[g_args]!, P[g]!.fsig.ret⟩,
+                  X[bbody.args]!, .codeOf P f bbody⟩}
 
   | promote {f unpr g prom X K c K'} :
     K.unpr = [] ->
     K'.prom = [] ->
-    Step Pr {K ⬝ ⟨f, ⟨g :: unpr, prom⟩, X, c⟩ ++ K'}
+    Step P {K ⬝ ⟨f, ⟨g :: unpr, prom⟩, X, c⟩ ++ K'}
             {K ⬝ ⟨f, ⟨unpr, g.ret :: prom⟩, X, c⟩ ++ K',
-             {⟨g.f, {}, g.args, codeEntry Pr g.f⟩}}
+             {⟨g.f, {}, g.args, .codeEntry P g.f⟩}}
 
   | spoin_unpr {f K ρ sc X bunpr bprom} :
-    Step Pr {K ⬝ ⟨f, ρ.push sc, X, .code (.trfr (.spoin bunpr bprom))⟩}
-            {K ⬝ ⟨f, ρ, X[bunpr.args]!, codeOf Pr f bunpr⟩}
+    Step P {K ⬝ ⟨f, ρ.push sc, X, .code (.spoin bunpr bprom)⟩}
+            {K ⬝ ⟨f, ρ, X[bunpr.args]!, .codeOf P f bunpr⟩}
 
   | spoin_prom {f K ρ X bunpr bprom Y y} {g : SpawnCall} :
     K.unpr = [] ->
-    Step Pr {(K ⬝ ⟨f, ⟨[], g.ret :: ρ⟩, X, .code (.trfr (.spoin bunpr bprom))⟩),
-             {⟨g.f, {}, Y, .code (.trfr (.retn y))⟩}}
-            {K ⬝ ⟨f, ⟨[], ρ⟩, X[bprom.args]! ++ Y[y]!, codeOf Pr f bprom⟩}
+    Step P {(K ⬝ ⟨f, ⟨[], g.ret :: ρ⟩, X, .code (.spoin bunpr bprom)⟩),
+             {⟨g.f, {}, Y, .code (.retn y)⟩}}
+            {K ⬝ ⟨f, ⟨[], ρ⟩, X[bprom.args]! ++ Y[y]!, .codeOf P f bprom⟩}
 
-inductive Steps (Pr : Program) : (P P' : ThreadPool) -> Type where
-  | nil {P : ThreadPool} : Steps Pr P P
-  | cons {P P' P'' : ThreadPool} : Steps Pr P P' -> Step Pr P' P'' -> Steps Pr P P''
+inductive Steps (P : Program) : (R R' : ThreadTree) -> Type where
+  | nil {R : ThreadTree} : Steps P R R
+  | cons {R R' R'' : ThreadTree} : Steps P R R' -> Step P R' R'' -> Steps P R R''
 
 namespace Step
-  notation (name := poolstep) Pr:arg " ⊢ " P:arg " ↦ " P':arg => Step Pr P P'
+  notation (name := poolstep) P:arg " ⊢ " R:arg " ↦ " R':arg => Step P R R'
 end Step
 
 namespace Steps
-  notation (name := stepsstep) Pr:arg " ⊢ " P:arg " ↦* " P':arg => Steps Pr P P'
+  notation (name := stepsstep) P:arg " ⊢ " R:arg " ↦* " R':arg => Steps P R R'
 
-  abbrev append {Pr : Program} : {P P' P'' : ThreadPool} ->
-                (Pr ⊢ P ↦* P') -> (Pr ⊢ P' ↦* P'') -> (Pr ⊢ P ↦* P'')
-    | _P, _P', .(_P'), ss', nil => ss'
-    | _P, _P', _P'', ss', cons ss s => cons (append ss' ss) s
-  instance instHAppend {Pr : Program} {P P' P'' : ThreadPool} :
-                       HAppend (Pr ⊢ P ↦* P') (Pr ⊢ P' ↦* P'') (Pr ⊢ P ↦* P'') where
+  @[simp] def append {P : Program} : {R R' R'' : ThreadTree} ->
+                (P ⊢ R ↦* R') -> (P ⊢ R' ↦* R'') -> (P ⊢ R ↦* R'')
+    | _R, _R', .(_R'), ss', nil => ss'
+    | _R, _R', _R'', ss', cons ss s => cons (append ss' ss) s
+  instance {P : Program} {R R' R'' : ThreadTree} :
+           HAppend (P ⊢ R ↦* R') (P ⊢ R' ↦* R'') (P ⊢ R ↦* R'') where
     hAppend := append
-  instance instSingleton {Pr : Program} {P P' : ThreadPool} : Singleton (Pr ⊢ P ↦ P') (Pr ⊢ P ↦* P') where
+  instance {P : Program} {R R' : ThreadTree} : Singleton (P ⊢ R ↦ R') (P ⊢ R ↦* R') where
     singleton := cons nil
 end Steps
-
-theorem codeOfGetElem {Pr : Program} {f : FuncIdx} {b : Cont}
-                    (pf : f < Pr.size) (pb : b.b < Pr.funs[f].blocks.length) :
-                    Pr.funs[f]!.blocks[b.b]! = Pr.funs[f].blocks[b.b] :=
-  by rw[getElem!_pos Pr.funs f pf, getElem!_pos Pr.funs[f].blocks b.b pb]
-
-theorem argsOfGetElem {x : List Var} {X : ValMap} (ok : IVec (·.Okay X.length) x):
-                    X[x]! = X[x] :=
-  getElem!_pos X x ok
