SporkProofs/Syntax.lean
@@ -1,5 +1,5 @@
---import Mathlib.Tactic.Linarith
 import SporkProofs.IVec
+import SporkProofs.HeadIs
 
 abbrev Val := Int
 
@@ -29,17 +29,14 @@ inductive Expr where
 inductive Cont where
   | mk (b : BlockIdx) (args : List Var)
 
-inductive Transfer where
+inductive Code where
+  | stmt (e : Expr) (c : Code)
   | goto (bnext : Cont)
   | ite (cond : Atom) (bthen : Cont) (belse : Cont)
   | call (f : FuncIdx) (args : List Var) (bret : Cont)
   | retn (args : List Var)
   | spork (bbody : Cont) (fspwn : FuncIdx) (args : List Var)
   | spoin (bunpr : Cont) (bprom : Cont)
-
-inductive Code where
-  | stmt (e : Expr) (c : Code)
-  | trfr (t : Transfer)
 
 abbrev SporkSig := List Nat
 
@@ -64,563 +61,575 @@ abbrev FuncSigs := List FuncSig
 abbrev BlockSigs := List BlockSig
 
 namespace BlockSig
-  abbrev arity | mk a _ss => a
-  abbrev sporkNest | mk _a ss => ss
-  abbrev bind | mk a ss => mk a.succ ss
-  abbrev spork | mk a ss, s => mk a (s :: ss)
-  abbrev spoin | mk a ss => mk a ss.tail
+  @[simp] abbrev arity | mk a _ss => a
+  @[simp] abbrev sporkNest | mk _a ss => ss
+  @[simp] abbrev bind | mk a ss => mk a.succ ss
+  @[simp] abbrev spork | mk a ss, s => mk a (s :: ss)
+  @[simp] abbrev spoin | mk a ss => mk a ss.tail
 
-  -- instance instDecidableEq : DecidableEq BlockSig
-  --   | ⟨ar, sn⟩, ⟨ar', sn'⟩ =>
-  --       decidable_of_iff ((ar, sn) = (ar', sn'))
-  --         ⟨congrArg (λ (areq, sneq) => mk areq sneq),
-  --          congrArg (λ | mk areq sneq => (areq, sneq))⟩
   deriving instance DecidableEq for BlockSig
+
+  @[simp] def add (a b : BlockSig) :=
+    mk (a.arity + b.arity) (a.sporkNest ++ b.sporkNest)
+
+  instance : Add BlockSig where
+    add := add
+
+  @[simp] theorem add_arity (a b : BlockSig) : (a + b).arity = a.arity + b.arity :=
+    by simp
+  @[simp] theorem add_sporkNest (a b : BlockSig) : (a + b).sporkNest = a.sporkNest ++ b.sporkNest :=
+    by simp
+  @[simp] theorem add_unfolded (a a' sn sn') : (mk a sn) + (mk a' sn') = mk (a + a') (sn ++ sn') :=
+    rfl
+  @[simp] theorem add_zero : (a : BlockSig) -> (a + .mk 0 []) = a
+    | .mk arity sn => by simp
 end BlockSig
 
 namespace FuncSig
-  abbrev arity | mk a _r => a
-  abbrev ret | mk _a r => r
+  @[simp] abbrev arity | mk a _r => a
+  @[simp] abbrev ret | mk _a r => r
 
-  -- instance instDecidableEq : DecidableEq FuncSig
-  --   | ⟨arity, ret⟩, ⟨arity', ret'⟩ =>
-  --     decidable_of_iff ((arity, ret) = (arity', ret'))
-  --       ⟨congrArg (λ (areq, sneq) => mk areq sneq),
-  --        congrArg (λ | mk areq sneq => (areq, sneq))⟩
   deriving instance DecidableEq, Inhabited for FuncSig
 end FuncSig
 
 namespace Var
-  variable (Γ : Scope)
+  @[simp] abbrev idx | mk v => v
 
-  abbrev idx | mk v => v
+  @[simp] abbrev inc | mk v, n => mk (v + n)
 
-  inductive Okay (v : Var) : Prop where
-    | mk : v.idx < Γ -> v.Okay
+  inductive WF (Γ : Scope) (v : Var) : Prop where
+    | mk : v.idx < Γ -> v.WF Γ
 
-  instance instDecidable (v : Var) : Decidable (v.Okay Γ) :=
-    decidable_of_iff (v.idx < Γ) ⟨(⟨·⟩), (·.1)⟩
+  namespace WF
+    theorem idx {Γ : Scope} {v : Var} : v.WF Γ -> v.idx < Γ | .mk idx => idx
+
+    instance {Γ : Scope} {v : Var} : Decidable (v.WF Γ) :=
+      decidable_of_iff (v.idx < Γ) ⟨(⟨·⟩), (·.1)⟩
+
+    theorem weakening {Γ Γ'} {v : Var} (wf : v.WF Γ) : v.WF (Γ + Γ') :=
+      .mk (Nat.lt_add_right Γ' wf.idx)
+  end WF
   
-  -- instance instDecidableEq : DecidableEq Var
-  --   | ⟨v⟩, ⟨v'⟩ => decidable_of_iff (v = v') ⟨congrArg mk, λ eq => congrArg (·.1) eq⟩
   deriving instance DecidableEq for Var
 
-  instance instOfNat {n} : OfNat Var n where
+  instance {n} : OfNat Var n where
     ofNat := Var.mk n
-  instance instCoeVarToNat : Coe Nat Var where
+  instance : Coe Nat Var where
     coe := mk
-  instance instCoeNatToVar : Coe Var Nat where
+  instance : Coe Var Nat where
     coe := idx
 end Var
 
 namespace Atom
-  variable (Γ : Scope)
+  inductive WF (Γ : Scope) : Atom -> Prop where
+    | val {v : Val} : (val v).WF Γ
+    | var {v : Var} : v.WF Γ -> (var v).WF Γ
 
-  inductive Okay : Atom -> Prop where
-    | val {v : Val} : (val v).Okay
-    | var {v : Var} : v.Okay Γ -> (var v).Okay
+  namespace WF
+    instance {Γ : Scope} : (a : Atom) -> Decidable (a.WF Γ)
+      | .val _v => isTrue val
+      | .var v => decidable_of_iff (v.WF Γ) ⟨var, λ (var v) => v⟩
 
-  instance instDecidable : (a : Atom) -> Decidable (a.Okay Γ)
-    | val _v => isTrue Okay.val
-    | var v => decidable_of_iff (v.Okay Γ) ⟨Okay.var, λ (.var v) => v⟩
+    theorem vwf {Γ : Scope} {v : Var} : (Atom.var v).WF Γ -> v.WF Γ | .var wf => wf
 
-  -- instance instDecidableEq : DecidableEq Atom
-  --   | val v, val v' => decidable_of_iff (v = v')
-  --       ⟨congrArg val, λ eq => congrArg (λ | (val v) => v | _ => v) eq⟩
-  --   | var v, var v' => decidable_of_iff (v = v')
-  --       ⟨congrArg var, λ eq => congrArg (λ | (var v) => v | _ => v) eq⟩
-  --   | val v, var v' => isFalse (by simp)
-  --   | var v, val v' => isFalse (by simp)
+    theorem weakening {Γ Γ'} {a : Atom} : a.WF Γ -> a.WF (Γ + Γ')
+      | .val => .val
+      | .var wf => .var wf.weakening
+  end WF
   deriving instance DecidableEq for Atom
 end Atom
 
 namespace Uop
-  -- instance instDecidableEq : DecidableEq Uop
-  --   | a, b => by cases a <;> cases b <;>
-  --                first | exact isTrue rfl | exact isFalse (by simp)
   deriving instance DecidableEq for Uop
 end Uop
 
 namespace Bop
-  -- instance instDecidableEq : DecidableEq Bop
-  --   | a, b => by cases a <;> cases b <;>
-  --                first | exact isTrue rfl | exact isFalse (by simp)
   deriving instance DecidableEq for Bop
 end Bop
 
-namespace Expr
-  variable (Γ : Scope)
-  
-  inductive Okay : Expr -> Prop where
-    | nop {a : Atom} : a.Okay Γ -> (nop a).Okay
-    | uop {o : Uop} {a : Atom} : a.Okay Γ -> (uop o a).Okay
-    | bop {o : Bop} {a b : Atom} : a.Okay Γ -> b.Okay Γ -> (bop o a b).Okay
+namespace Expr  
+  inductive WF (Γ : Scope) : Expr -> Prop where
+    | nop {a : Atom} : a.WF Γ -> (nop a).WF Γ
+    | uop {o : Uop} {a : Atom} : a.WF Γ -> (uop o a).WF Γ
+    | bop {o : Bop} {a b : Atom} : a.WF Γ -> b.WF Γ -> (bop o a b).WF Γ
 
-  instance instDecidable : (e : Expr) -> Decidable (e.Okay Γ)
-    | nop a => decidable_of_iff (a.Okay Γ)
-        ⟨Okay.nop, λ (.nop a) => a⟩
-    | uop _o a => decidable_of_iff (a.Okay Γ)
-        ⟨Okay.uop, λ (.uop ok) => ok⟩
-    | bop _o a b => decidable_of_iff (a.Okay Γ ∧ b.Okay Γ)
-        ⟨And.elim Okay.bop, λ (.bop a b) => ⟨a, b⟩⟩
+  namespace WF
+    instance {Γ : Scope} : (e : Expr) -> Decidable (e.WF Γ)
+      | .nop a => decidable_of_iff (a.WF Γ)
+          ⟨nop, λ (nop a) => a⟩
+      | .uop _o a => decidable_of_iff (a.WF Γ)
+          ⟨uop, λ (uop wf) => wf⟩
+      | .bop _o a b => decidable_of_iff (a.WF Γ ∧ b.WF Γ)
+          ⟨And.elim bop, λ (bop a b) => ⟨a, b⟩⟩
 
-  -- instance instDecidableEq : DecidableEq Expr
-  --   | nop v, nop v' =>
-  --     decidable_of_iff (v = v')
-  --       ⟨congrArg nop,
-  --        congrArg (λ | nop v => v | _ => v)⟩
-  --   | uop o a, uop o' a' =>
-  --     decidable_of_iff ((o, a) = (o', a'))
-  --       ⟨congrArg (λ (o, a) => uop o a),
-  --        congrArg (λ | uop o a => (o, a) | _ => (o, a))⟩
-  --   | bop o a b, bop o' a' b' =>
-  --     decidable_of_iff ((o, a, b) = (o', a', b'))
-  --       ⟨congrArg (λ (o, a, b) => bop o a b),
-  --        congrArg (λ | bop o a b => (o, a, b) | _ => (o, a, b))⟩
-  --   | nop _, uop _ _ => isFalse (by simp)
-  --   | nop _, bop _ _ _ => isFalse (by simp)
-  --   | uop _ _, nop _ => isFalse (by simp)
-  --   | uop _ _, bop _ _ _ => isFalse (by simp)
-  --   | bop _ _ _, nop _ => isFalse (by simp)
-  --   | bop _ _ _, uop _ _ => isFalse (by simp)
+    theorem weakening {Γ Γ'} {e : Expr} : e.WF Γ -> e.WF (Γ + Γ')
+      | .nop a => .nop a.weakening
+      | .uop a => .uop a.weakening
+      | .bop a b => .bop a.weakening b.weakening
+  end WF
+
   deriving instance DecidableEq for Expr
 end Expr
 
 namespace Cont
-  variable
-    (bsigs : BlockSigs)
-    (bsig : BlockSig)
-
-  abbrev b | mk b _args => b
-  abbrev args | mk _b args => args
+  @[simp] abbrev b | mk b _args => b
+  @[simp] abbrev args | mk _b args => args
 
   -- a continuation that takes `bsig.arity + rets` args
-  inductive OkayRets (rets : Nat) (b : Cont) :Prop where
+  inductive WFRets (bsigs : BlockSigs) (bsig : BlockSig) (rets : Nat) (b : Cont) : Prop where
     | mk (_ : b.b < bsigs.length)
          (_ : bsigs[b.b] = ⟨b.args.length + rets, bsig.sporkNest⟩)
-         (_ : IVec (·.Okay bsig.arity) b.args)
+         (_ : IVec (·.WF bsig.arity) b.args)
 
-  inductive Okay (b : Cont) : Prop where
+  inductive WF (bsigs : BlockSigs) (bsig : BlockSig) (b : Cont) : Prop where
     | mk (_ : b.b < bsigs.length)
          (_ : bsigs[b.b] = ⟨b.args.length, bsig.sporkNest⟩)
-         (_ : IVec (·.Okay bsig.arity) b.args)
+         (_ : IVec (·.WF bsig.arity) b.args)
 
-  instance instOkayRetsOkayCoe {bsigs : BlockSigs} {bsig : BlockSig} {b : Cont} :
-                               Coe (OkayRets bsigs bsig 0 b) (Okay bsigs bsig b) where
-    coe := λ  ⟨bok, blen, argsok⟩ => ⟨bok, blen, argsok⟩
-  instance instOkayOkayRetsCoe {bsigs : BlockSigs} {bsig : BlockSig} {b : Cont} :
-                               Coe (Okay bsigs bsig b) (OkayRets bsigs bsig 0 b) where
-    coe := λ ⟨bok, blen, argsok⟩ => ⟨bok, blen, argsok⟩
+  namespace WFRets
+    instance {bsigs : BlockSigs} {bsig : BlockSig} {b : Cont} :
+             Coe (WFRets bsigs bsig 0 b) (WF bsigs bsig b) where
+      coe := λ ⟨bwf, blen, argswf⟩ => ⟨bwf, blen, argswf⟩
 
-  namespace OkayRets
-    abbrev cast0 {bsigs bsig b} : OkayRets bsigs bsig 0 b -> Okay bsigs bsig b
+    instance {bsigs : BlockSigs} {bsig : BlockSig} {rets : Nat} {b : Cont} : Decidable (b.WFRets bsigs bsig rets) :=
+      dite (b.b < bsigs.length)
+        (λ t => decidable_of_iff
+                  ((bsigs[b.b] = ⟨b.args.length + rets, bsig.sporkNest⟩) ∧
+                   IVec (·.WF bsig.arity) b.args)
+                  ⟨λ ⟨p1, p2⟩ => ⟨t, p1, p2⟩,
+                   λ ⟨_, p1, p2⟩ => ⟨p1, p2⟩⟩)
+        (λ f => isFalse (f ∘ (λ ⟨p, _, _⟩ => p)))
+
+    abbrev cast0 {bsigs bsig b} : WFRets bsigs bsig 0 b -> WF bsigs bsig b
       | ⟨a, b, c⟩ => ⟨a, b, c⟩
-  end OkayRets
+    theorem blt {bsigs bsig rets b} (wf : WFRets bsigs bsig rets b) :
+                b.b < bsigs.length := wf.1
+    theorem bsig {bsigs bsig rets b} (wf : WFRets bsigs bsig rets b) :
+                 bsigs[b.b]'wf.blt = ⟨b.args.length + rets, bsig.sporkNest⟩ := wf.2
+    theorem args {bsigs bsig rets b} (wf : WFRets bsigs bsig rets b) :
+                 IVec (·.WF bsig.arity) b.args := wf.3
 
-  namespace Okay
-    abbrev cast0 {bsigs bsig b} : Okay bsigs bsig b -> OkayRets bsigs bsig 0 b
+    theorem weakening_bsigs
+            {bsigs bsigs' bsig ret b} :
+            WFRets bsigs bsig ret b ->
+            WFRets (bsigs ++ bsigs') bsig ret b
+      | mk blt bsigb args =>
+        mk (List.length_append ▸ Nat.lt_add_right bsigs'.length blt)
+           (List.getElem_append_left' blt bsigs' ▸ bsigb)
+           args
+  end WFRets
+
+  namespace WF
+    instance {bsigs : BlockSigs} {bsig : BlockSig} {b : Cont} :
+             Coe (WF bsigs bsig b) (WFRets bsigs bsig 0 b) where
+      coe := λ ⟨bwf, blen, argswf⟩ => ⟨bwf, blen, argswf⟩
+
+    instance {bsigs : BlockSigs} {bsig : BlockSig} {b : Cont} : Decidable (b.WF bsigs bsig) :=
+      decidable_of_iff (b.WFRets bsigs bsig 0) ⟨Coe.coe, Coe.coe⟩
+
+    abbrev cast0 {bsigs bsig b} : WF bsigs bsig b -> WFRets bsigs bsig 0 b
       | ⟨a, b, c⟩ => ⟨a, b, c⟩
-  end Okay
+    theorem blt {bsigs bsig b} (wf : WF bsigs bsig b) :
+                b.b < bsigs.length := wf.1
+    theorem bsig {bsigs bsig b} (wf : WF bsigs bsig b) :
+                 bsigs[b.b]'wf.blt = ⟨b.args.length, bsig.sporkNest⟩ := wf.2
+    theorem args {bsigs bsig b} (wf : WF bsigs bsig b) :
+                 IVec (·.WF bsig.arity) b.args := wf.3
 
-  def OkayRets0_iff_Okay {bsigs : BlockSigs} {bsig : BlockSig} {b : Cont} :
-                         OkayRets bsigs bsig 0 b ↔ Okay bsigs bsig b :=
+    theorem weakening_bsigs
+            {bsigs bsigs' bsig b}
+            (wf : WF bsigs bsig b) :
+            WF (bsigs ++ bsigs') bsig b :=
+      wf.cast0.weakening_bsigs.cast0
+  end WF
+
+  theorem WFRets0_iff_WF {bsigs : BlockSigs} {bsig : BlockSig} {b : Cont} :
+                         WFRets bsigs bsig 0 b ↔ WF bsigs bsig b :=
     ⟨Coe.coe, Coe.coe⟩
 
-  instance instDecidableRets (rets : Nat) (b : Cont) : Decidable (b.OkayRets bsigs bsig rets) :=
-    dite (b.b < bsigs.length)
-      (λ t => decidable_of_iff
-                ((bsigs[b.b] = ⟨b.args.length + rets, bsig.sporkNest⟩) ∧
-                 IVec (·.Okay bsig.arity) b.args)
-                ⟨λ ⟨p1, p2⟩ => ⟨t, p1, p2⟩,
-                 λ ⟨_, p1, p2⟩ => ⟨p1, p2⟩⟩)
-      (λ f => isFalse (f ∘ (λ ⟨p, _, _⟩ => p)))
-
-  instance instDecidable (b : Cont) : Decidable (b.Okay bsigs bsig) :=
-    decidable_of_iff (b.OkayRets bsigs bsig 0) OkayRets0_iff_Okay
-
-  -- instance instDecidableEq : DecidableEq Cont
-  --   | ⟨b, args⟩, ⟨b', args'⟩ => decidable_of_iff
-  --       ((b, args) = (b', args'))
-  --       ⟨congrArg (λ (b, args) => mk b args),
-  --        congrArg (λ | mk b args => (b, args))⟩
   deriving instance DecidableEq for Cont
 end Cont
 
-namespace Transfer
-  variable
-    (fsigs : FuncSigs)
-    (bsigs : BlockSigs)
-    (ret : Nat)
-    (bsig : BlockSig)
+namespace Code
+  --notation e:arg " ;; " c => stmt e c
 
-  inductive Okay : Transfer -> Prop where
+  inductive WF (fsigs : FuncSigs) (bsigs ret) : BlockSig -> Code -> Prop where
+    | stmt
+        {bsig : BlockSig}
+        {e : Expr}
+        {c : Code} :
+        e.WF bsig.arity ->
+        c.WF fsigs bsigs ret bsig.bind ->
+        (stmt e c).WF fsigs bsigs ret bsig
+
     | goto
+        {bsig : BlockSig}
         {bnext : Cont} :
-        bnext.Okay bsigs bsig ->
-        (goto bnext).Okay
+        bnext.WF bsigs bsig ->
+        (goto bnext).WF fsigs bsigs ret bsig
 
     | ite
+        {bsig : BlockSig}
         {cond : Atom}
         {bthen : Cont}
         {belse : Cont} :
-        cond.Okay bsig.arity ->
-        bthen.Okay bsigs bsig ->
-        belse.Okay bsigs bsig ->
-        (ite cond bthen belse).Okay
+        cond.WF bsig.arity ->
+        bthen.WF bsigs bsig ->
+        belse.WF bsigs bsig ->
+        (ite cond bthen belse).WF fsigs bsigs ret bsig
 
     | call
+        {bsig : BlockSig}
         {f : FuncIdx}
         {args : List Var}
         {bret : Cont} :
         (_ : f < fsigs.length) ->
         fsigs[f].arity = args.length ->
-        IVec (·.Okay bsig.arity) args ->
-        bret.OkayRets bsigs bsig fsigs[f].ret ->
-        (call f args bret).Okay
+        IVec (·.WF bsig.arity) args ->
+        bret.WFRets bsigs bsig fsigs[f].ret ->
+        (call f args bret).WF fsigs bsigs ret bsig
         
     | retn
+        {bsig : BlockSig}
         {args : List Var} :
         bsig.sporkNest = [] ->
         ret = args.length ->
-        IVec (·.Okay bsig.arity) args ->
-        (retn args).Okay
+        IVec (·.WF bsig.arity) args ->
+        (retn args).WF fsigs bsigs ret bsig
 
     | spork
+        {bsig : BlockSig}
         {bbody : Cont}
         {fspwn : FuncIdx}
         {args : List Var} :
         (_ : fspwn < fsigs.length) ->
         fsigs[fspwn].arity = args.length ->
-        IVec (·.Okay bsig.arity) args ->
-        bbody.Okay bsigs (bsig.spork fsigs[fspwn].ret) ->
-        (spork bbody fspwn args).Okay
+        IVec (·.WF bsig.arity) args ->
+        bbody.WF bsigs (bsig.spork fsigs[fspwn].ret) ->
+        (spork bbody fspwn args).WF fsigs bsigs ret bsig
 
     | spoin
+        {bsig : BlockSig}
         {bunpr : Cont}
         {bprom : Cont} :
         (bsig_sn_nonnil : bsig.sporkNest ≠ []) ->
-        bunpr.Okay bsigs bsig.spoin ->
-        bprom.OkayRets bsigs bsig.spoin (bsig.sporkNest.head bsig_sn_nonnil) ->
-        (spoin bunpr bprom).Okay
+        bunpr.WF bsigs bsig.spoin ->
+        bprom.WFRets bsigs bsig.spoin (bsig.sporkNest.head bsig_sn_nonnil) ->
+        (spoin bunpr bprom).WF fsigs bsigs ret bsig
 
-  namespace Okay
+
+  @[simp] def split : Code -> List Expr × (c : Code) ×' (∀ e, ∀ c', c ≠ .stmt e c')
+    | stmt e c => let (es, cp) := c.split; (e :: es, cp)
+    | goto bnext => ([], ⟨goto bnext, by intros e c; simp⟩)
+    | ite e bthen belse => ([], ⟨ite e bthen belse, by intros e c; simp⟩)
+    | call g args bret => ([], ⟨call g args bret, by intros e c; simp⟩)
+    | retn args => ([], ⟨retn args, by intros e c; simp⟩)
+    | spork bbody gspwn gargs => ([], ⟨spork bbody gspwn gargs, by intros e c; simp⟩)
+    | spoin bunpr bprom => ([], ⟨spoin bunpr bprom, by intros e c; simp⟩)
+
+  @[simp] def join : List Expr -> Code -> Code
+    | [], c => c
+    | e :: es, c => stmt e (join es c)
+
+  @[simp] theorem join_split {c e c' p} (q : split c = (e, ⟨c', p⟩)) : join e c' = c := by
+    cases c <;> try (cases e <;> simp_all)
+    · case stmt e' es' e'' es'' =>
+      exact join_split (Prod.ext q.1.2 q.2)
+
+  namespace WF
+    instance instDecidable {fsigs bsigs ret bsig} : (c : Code) ->
+                           Decidable (c.WF fsigs bsigs ret bsig)
+      | .stmt e c =>
+          let _ : Decidable (c.WF fsigs bsigs ret bsig.bind) := instDecidable c
+          decidable_of_iff (e.WF bsig.arity ∧ c.WF fsigs bsigs ret bsig.bind)
+            ⟨λ ⟨e, c⟩ => stmt e c, λ | stmt e c => ⟨e, c⟩⟩
+      | .goto bnext =>
+          decidable_of_iff (bnext.WF bsigs bsig)
+            ⟨goto, λ | goto wf => wf⟩
+      | .ite cond bthen belse =>
+          decidable_of_iff (cond.WF bsig.arity ∧ bthen.WF bsigs bsig ∧ belse.WF bsigs bsig)
+            ⟨λ ⟨a, b, c⟩ => ite a b c, λ | ite a b c => ⟨a, b, c⟩⟩
+      | .call f args bret =>
+          decidable_of_iff (∃ _ : f < fsigs.length,
+                            fsigs[f].arity = args.length ∧
+                            IVec (·.WF bsig.arity) args ∧
+                            bret.WFRets bsigs bsig fsigs[f].ret)
+            ⟨λ ⟨a, b, c, d⟩ => call a b c d,
+             λ | call a b c d => ⟨a, b, c, d⟩⟩
+      | .retn args =>
+          decidable_of_iff (bsig.sporkNest = [] ∧ ret = args.length ∧ IVec (·.WF bsig.arity) args)
+            ⟨λ ⟨a, b, c⟩ => retn a b c, λ | retn a b c => ⟨a, b, c⟩⟩
+      | .spork bbody fspwn args =>
+          decidable_of_iff (∃ _ : fspwn < fsigs.length,
+                            fsigs[fspwn].arity = args.length ∧
+                            IVec (·.WF bsig.arity) args ∧
+                            bbody.WF bsigs (bsig.spork fsigs[fspwn].ret))
+            ⟨λ ⟨a, b, c, d⟩ => spork a b c d, λ | spork a b c d => ⟨a, b, c, d⟩⟩
+      | .spoin bunpr bprom =>
+          match (generalizing := true) h : bsig with
+            | ⟨arity, []⟩ =>
+                isFalse (λ x => by cases x <;> contradiction)
+            | ⟨arity, s :: ss⟩ =>
+                decidable_of_iff (bunpr.WF bsigs ⟨arity, ss⟩ ∧
+                                  bprom.WFRets bsigs ⟨arity, ss⟩ s)
+                ⟨λ ⟨a, b⟩ => spoin (by simp) a b,
+                 λ | spoin h' a b => ⟨a, b⟩⟩
+
     -- Accessor methods
-    theorem goto_bnext {bnext} :
-                       Okay fsigs bsigs ret bsig (.goto bnext) ->
-                       bnext.Okay bsigs bsig
-      | .goto bnextₒₖ => bnextₒₖ
+    theorem stmt_expr {fsigs bsigs ret bsig e c} : (Code.stmt e c).WF fsigs bsigs ret bsig -> e.WF bsig.arity
+      | stmt ewf _cwf => ewf
+    theorem stmt_code {fsigs bsigs ret bsig e c} : (Code.stmt e c).WF fsigs bsigs ret bsig -> c.WF fsigs bsigs ret bsig.bind
+      | stmt _ewf cwf => cwf
 
-    theorem ite_cond {cond bthen belse} :
-                     Okay fsigs bsigs ret bsig (.ite cond bthen belse) ->
-                     cond.Okay bsig.arity
-      | .ite condₒₖ _ _ => condₒₖ
-    theorem ite_bthen {cond bthen belse} :
-                      Okay fsigs bsigs ret bsig (.ite cond bthen belse) ->
-                      bthen.Okay bsigs bsig
-      | .ite _ bthenₒₖ _ => bthenₒₖ
-    theorem ite_belse {cond bthen belse} :
-                      Okay fsigs bsigs ret bsig (.ite cond bthen belse) ->
-                      belse.Okay bsigs bsig
-      | .ite _ _ belseₒₖ => belseₒₖ
+    theorem goto_bnext {fsigs bsigs ret bsig bnext} :
+                       WF fsigs bsigs ret bsig (.goto bnext) ->
+                       bnext.WF bsigs bsig
+      | goto bnextwf => bnextwf
 
-    theorem call_flt {f args bret} :
-                     Okay fsigs bsigs ret bsig (.call f args bret) ->
+    theorem ite_cond {fsigs bsigs ret bsig cond bthen belse} :
+                     WF fsigs bsigs ret bsig (.ite cond bthen belse) ->
+                     cond.WF bsig.arity
+      | ite condwf _ _ => condwf
+    theorem ite_bthen {fsigs bsigs ret bsig cond bthen belse} :
+                      WF fsigs bsigs ret bsig (.ite cond bthen belse) ->
+                      bthen.WF bsigs bsig
+      | ite _ bthenwf _ => bthenwf
+    theorem ite_belse {fsigs bsigs ret bsig cond bthen belse} :
+                      WF fsigs bsigs ret bsig (.ite cond bthen belse) ->
+                      belse.WF bsigs bsig
+      | ite _ _ belsewf => belsewf
+
+    theorem call_flt {fsigs bsigs ret bsig f args bret} :
+                     WF fsigs bsigs ret bsig (.call f args bret) ->
                      f < fsigs.length
-      | .call flt _ _ _ => flt
-    theorem call_arity {f args bret} :
-                       (ok : Okay fsigs bsigs ret bsig (.call f args bret)) ->
-                       (fsigs[f]'ok.call_flt).arity = args.length
-      | .call _ arityₒₖ _ _ => arityₒₖ
-    theorem call_args {f args bret} :
-                      Okay fsigs bsigs ret bsig (.call f args bret) ->
-                      IVec (·.Okay bsig.arity) args
-      | .call _ _ argsₒₖ _ => argsₒₖ
-    theorem call_bret {f args bret} :
-                      (ok : Okay fsigs bsigs ret bsig (.call f args bret)) ->
-                      bret.OkayRets bsigs bsig (fsigs[f]'ok.call_flt).ret
-      | .call _ _ _ bretₒₖ => bretₒₖ
+      | call flt _ _ _ => flt
+    theorem call_arity {fsigs bsigs ret bsig f args bret} :
+                       (wf : WF fsigs bsigs ret bsig (.call f args bret)) ->
+                       (fsigs[f]'wf.call_flt).arity = args.length
+      | call _ aritywf _ _ => aritywf
+    theorem call_args {fsigs bsigs ret bsig f args bret} :
+                      WF fsigs bsigs ret bsig (.call f args bret) ->
+                      IVec (·.WF bsig.arity) args
+      | call _ _ argswf _ => argswf
+    theorem call_bret {fsigs bsigs ret bsig f args bret} :
+                      (wf : WF fsigs bsigs ret bsig (.call f args bret)) ->
+                      bret.WFRets bsigs bsig (fsigs[f]'wf.call_flt).ret
+      | call _ _ _ bretwf => bretwf
 
-    theorem retn_sn_nil {args} :
-                          Okay fsigs bsigs ret bsig (.retn args) ->
+    theorem retn_sn_nil {fsigs bsigs ret bsig args} :
+                          WF fsigs bsigs ret bsig (.retn args) ->
                           bsig.sporkNest = []
-      | .retn n _ _ => n
-    theorem retn_length {args} :
-                        Okay fsigs bsigs ret bsig (.retn args) ->
+      | retn n _ _ => n
+    theorem retn_length {fsigs bsigs ret bsig args} :
+                        WF fsigs bsigs ret bsig (.retn args) ->
                         ret = args.length
-      | .retn _ l _ => l
-    theorem retn_args {args} :
-                      Okay fsigs bsigs ret bsig (.retn args) ->
-                      IVec (·.Okay bsig.arity) args
-      | .retn _ _ a => a
+      | retn _ l _ => l
+    theorem retn_args {fsigs bsigs ret bsig args} :
+                      WF fsigs bsigs ret bsig (.retn args) ->
+                      IVec (·.WF bsig.arity) args
+      | retn _ _ a => a
 
-    theorem spork_flt {bbody f args} :
-                      Okay fsigs bsigs ret bsig (.spork bbody f args) ->
+    theorem spork_flt {fsigs bsigs ret bsig bbody f args} :
+                      WF fsigs bsigs ret bsig (.spork bbody f args) ->
                       f < fsigs.length
-      | .spork flt _ _ _ => flt
-    theorem spork_arity {bbody f args} :
-                        (ok : Okay fsigs bsigs ret bsig (.spork bbody f args)) ->
-                        (fsigs[f]'ok.spork_flt).arity = args.length
-      | .spork _ arityₒₖ _ _ => arityₒₖ
-    theorem spork_args {bbody f args} :
-                      Okay fsigs bsigs ret bsig (.spork bbody f args) ->
-                      IVec (·.Okay bsig.arity) args
-      | .spork _ _ argsₒₖ _ => argsₒₖ
-    theorem spork_bbody {bbody f args} :
-                        (ok : Okay fsigs bsigs ret bsig (.spork bbody f args)) ->
-                        bbody.Okay bsigs (bsig.spork (fsigs[f]'ok.spork_flt).ret)
-      | .spork _ _ _ bbodyₒₖ => bbodyₒₖ
+      | spork flt _ _ _ => flt
+    theorem spork_arity {fsigs bsigs ret bsig bbody f args} :
+                        (wf : WF fsigs bsigs ret bsig (.spork bbody f args)) ->
+                        (fsigs[f]'wf.spork_flt).arity = args.length
+      | spork _ aritywf _ _ => aritywf
+    theorem spork_args {fsigs bsigs ret bsig bbody f args} :
+                      WF fsigs bsigs ret bsig (.spork bbody f args) ->
+                      IVec (·.WF bsig.arity) args
+      | spork _ _ argswf _ => argswf
+    theorem spork_bbody {fsigs bsigs ret bsig bbody f args} :
+                        (wf : WF fsigs bsigs ret bsig (.spork bbody f args)) ->
+                        bbody.WF bsigs (bsig.spork (fsigs[f]'wf.spork_flt).ret)
+      | spork _ _ _ bbodywf => bbodywf
 
-    theorem spoin_sn_nonnil {bunpr bprom} :
-                            Okay fsigs bsigs ret bsig (.spoin bunpr bprom) ->
+    theorem spoin_sn_nonnil {fsigs bsigs ret bsig bunpr bprom} :
+                            WF fsigs bsigs ret bsig (.spoin bunpr bprom) ->
                             bsig.sporkNest ≠ []
-      | .spoin nn _ _ => nn
-    theorem spoin_bunpr {bunpr bprom} :
-                        Okay fsigs bsigs ret bsig (.spoin bunpr bprom) ->
-                        bunpr.Okay bsigs bsig.spoin
-      | .spoin _ bunprₒₖ _ => bunprₒₖ
-    theorem spoin_bprom {bunpr bprom} :
-                        (ok : Okay fsigs bsigs ret bsig (.spoin bunpr bprom)) ->
-                        bprom.OkayRets bsigs bsig.spoin
-                          (bsig.sporkNest.head ok.spoin_sn_nonnil)
-      | .spoin _ _ bpromₒₖ => bpromₒₖ
-  end Okay
+      | spoin nn _ _ => nn
+    theorem spoin_bunpr {fsigs bsigs ret bsig bunpr bprom} :
+                        WF fsigs bsigs ret bsig (.spoin bunpr bprom) ->
+                        bunpr.WF bsigs bsig.spoin
+      | spoin _ bunprwf _ => bunprwf
+    theorem spoin_bprom {fsigs bsigs ret bsig bunpr bprom} :
+                        (wf : WF fsigs bsigs ret bsig (.spoin bunpr bprom)) ->
+                        bprom.WFRets bsigs bsig.spoin
+                          (bsig.sporkNest.head wf.spoin_sn_nonnil)
+      | spoin _ _ bpromwf => bpromwf
 
-  instance instDecidable : (t : Transfer) -> Decidable (t.Okay fsigs bsigs ret bsig)
-    | goto bnext =>
-        decidable_of_iff (bnext.Okay bsigs bsig)
-          ⟨Okay.goto, λ | .goto ok => ok⟩
-    | ite cond bthen belse =>
-        decidable_of_iff (cond.Okay bsig.arity ∧ bthen.Okay bsigs bsig ∧ belse.Okay bsigs bsig)
-          ⟨λ ⟨a, b, c⟩ => Okay.ite a b c, λ | .ite a b c => ⟨a, b, c⟩⟩
-    | call f args bret =>
-        decidable_of_iff (∃ _ : f < fsigs.length,
-                          fsigs[f].arity = args.length ∧
-                          IVec (·.Okay bsig.arity) args ∧
-                          bret.OkayRets bsigs bsig fsigs[f].ret)
-          ⟨λ ⟨a, b, c, d⟩ => Okay.call a b c d,
-           λ | .call a b c d => ⟨a, b, c, d⟩⟩
-    | retn args =>
-        decidable_of_iff (bsig.sporkNest = [] ∧ ret = args.length ∧ IVec (·.Okay bsig.arity) args)
-          ⟨λ ⟨a, b, c⟩ => Okay.retn a b c, λ | .retn a b c => ⟨a, b, c⟩⟩
-    | spork bbody fspwn args =>
-        decidable_of_iff (∃ _ : fspwn < fsigs.length,
-                          fsigs[fspwn].arity = args.length ∧
-                          IVec (·.Okay bsig.arity) args ∧
-                          bbody.Okay bsigs (bsig.spork fsigs[fspwn].ret))
-          ⟨λ ⟨a, b, c, d⟩ => Okay.spork a b c d, λ | .spork a b c d => ⟨a, b, c, d⟩⟩
-    | spoin bunpr bprom =>
-        match (generalizing := true) h : bsig with
-          | ⟨arity, []⟩ => isFalse (λ x => by cases x; contradiction)
-          | ⟨arity, s :: ss⟩ =>
-              decidable_of_iff (bunpr.Okay bsigs ⟨arity, ss⟩ ∧
-                                bprom.OkayRets bsigs ⟨arity, ss⟩ s)
-              ⟨λ ⟨a, b⟩ => Okay.spoin (by simp) a b,
-               λ | .spoin h' a b => ⟨a, b⟩⟩
+    theorem weakening_bsigs
+            {fsigs bsigs bsigs' ret bsig c} :
+            WF fsigs bsigs ret bsig c ->
+            WF fsigs (bsigs ++ bsigs') ret bsig c
+      | stmt ewf cwf =>
+        stmt ewf cwf.weakening_bsigs
+      | goto bnextwf =>
+        goto bnextwf.weakening_bsigs
+      | ite ewf bthenwf belsewf =>
+        ite ewf bthenwf.weakening_bsigs belsewf.weakening_bsigs
+      | call flt aritywf argswf bretwf =>
+        call flt aritywf argswf bretwf.weakening_bsigs
+      | retn snwf retwf argswf =>
+        retn snwf retwf argswf
+      | spork flt aritywf argswf bbodywf =>
+        spork flt aritywf argswf bbodywf.weakening_bsigs
+      | spoin snwf bunprwf bpromwf =>
+        spoin snwf bunprwf.weakening_bsigs bpromwf.weakening_bsigs
 
-  -- instance instDecidableEq : DecidableEq Transfer
-  --   | t, t' => by
-  --     cases t <;> cases t' <;>
+    theorem join_wf {fsigs bsigs ret bsig} :
+            {e : List Expr} -> {c : Code} ->
+            (∀ i : Fin e.length, e[i].WF (bsig.arity + i)) ->
+            c.WF fsigs bsigs ret (bsig + .mk e.length []) ->
+            (c.join e).WF fsigs bsigs ret bsig
+      | [], c, ewf, cwf => by simpa using cwf
+      | e :: es, c, ewf, cwf =>
+        .stmt (ewf ⟨0, by simp⟩)
+          (join_wf (bsig := bsig.bind) (e := es)
+            (λ i => let ewf' := ewf ⟨i.1 + 1, by simp⟩
+                    by simp[← Nat.add_assoc bsig.1 1 i.1] at ewf'
+                       simp
+                       rw[Nat.add_assoc, Nat.add_comm 1 i.1]
+                       exact ewf')
+            (match bsig with
+              | .mk arity sn => by
+                simp
+                simp at cwf
+                rw[Nat.add_comm es.length 1,
+                   ← Nat.add_assoc] at cwf
+                exact cwf))
 
-  --     -- for mismatched constructors, automatically
-  --     -- derive isFalse by contradiction:
-  --     try (apply isFalse; intro; contradiction)
+    theorem split_wf {fsigs bsigs ret bsig} {c : Code} (cwf : c.WF fsigs bsigs ret bsig) :
+            (∀ i : Fin c.split.1.length, c.split.1[i].WF (bsig.arity + i))
+              ∧ c.split.2.1.WF fsigs bsigs ret (bsig + .mk c.split.1.length []) := by
+      cases c <;> try (exact And.intro (λ i => nomatch i) (by simpa using cwf))
+      · case stmt e c =>
+        let p := @split_wf fsigs bsigs ret bsig.bind c cwf.stmt_code
+        apply And.intro
+        · exact (λ | ⟨0, l⟩ => cwf.stmt_expr
+                   | ⟨i + 1, l⟩ =>
+                     by simpa[Nat.add_assoc, Nat.add_comm 1 i]
+                        using p.1 ⟨i, by simpa using l⟩)
+        · (match h : bsig with
+             | .mk arity sn =>
+               simpa[h, Nat.add_assoc, Nat.add_comm 1]
+               using p.2)
+  end WF
 
-  --     -- remaining cases, potentially isTrue:
-  --     · case goto.goto bnext bnext' =>
-  --         exact decidable_of_iff (bnext = bnext')
-  --           ⟨congrArg goto,
-  --            congrArg (λ | goto bnext => bnext | _ => bnext)⟩
-
-  --     · case ite.ite cond bthen belse cond' bthen' belse' =>
-  --         exact decidable_of_iff ((cond, bthen, belse) = (cond', bthen', belse'))
-  --           ⟨congrArg (λ (a, b, c) => ite a b c),
-  --            congrArg (λ | ite a b c => (a, b, c) | _ => (cond, bthen, belse))⟩
-
-  --     · case call.call f args bret f' args' bret' =>
-  --         exact decidable_of_iff ((f, args, bret) = (f', args', bret'))
-  --           ⟨congrArg (λ (a, b, c) => call a b c),
-  --            congrArg (λ | call f args bret => (f, args, bret) | _ => (f, args, bret))⟩
-
-  --     · case retn.retn args args' =>
-  --         exact decidable_of_iff (args = args')
-  --           ⟨congrArg retn,
-  --            congrArg (λ | retn args => args | _ => args)⟩
-
-  --     · case spork.spork bbody fspwn args bbody' fspwn' args' =>
-  --         exact decidable_of_iff ((bbody, fspwn, args) = (bbody', fspwn', args'))
-  --           ⟨congrArg (λ (a, b, c) => spork a b c),
-  --            congrArg (λ | spork a b c => (a, b, c) | _ => (bbody, fspwn, args))⟩
-
-  --     · case spoin.spoin bunpr bprom bunpr' bprom' =>
-  --         exact decidable_of_iff ((bunpr, bprom) = (bunpr', bprom'))
-  --           ⟨congrArg (λ (a, b) => spoin a b),
-  --            congrArg (λ | spoin a b => (a, b) | _ => (bunpr, bprom))⟩
-  deriving instance DecidableEq for Transfer
-end Transfer
-
-namespace Code
-  variable
-    (fsigs : FuncSigs)
-    (bsigs : BlockSigs)
-    (ret : Nat)
-
-  abbrev view : Code -> List Expr × Transfer
-    | stmt e c => let (es, t) := view c; (e :: es, t)
-    | trfr t => ([], t)
-
-  inductive Okay : (bsig : BlockSig) -> Code -> Prop where
-    | stmt
-        {bsig : BlockSig}
-        {e : Expr}
-        {c : Code} :
-        e.Okay bsig.arity ->
-        c.Okay bsig.bind ->
-        (stmt e c).Okay bsig
-
-    | trfr
-        {bsig : BlockSig}
-        {t : Transfer} :
-        t.Okay fsigs bsigs ret bsig ->
-        (trfr t).Okay bsig
-
-  namespace Okay
-    abbrev t {fsigs bsigs ret bsig t} : (Code.trfr t).Okay fsigs bsigs ret bsig -> t.Okay fsigs bsigs ret bsig
-      | trfr ok => ok
-    abbrev e {fsigs bsigs ret bsig e c} : (Code.stmt e c).Okay fsigs bsigs ret bsig -> e.Okay bsig.arity
-      | stmt eok _cok => eok
-    abbrev c {fsigs bsigs ret bsig e c} : (Code.stmt e c).Okay fsigs bsigs ret bsig -> c.Okay fsigs bsigs ret bsig.bind
-      | stmt _eok cok => cok
-  end Okay
-
-  instance instDecidable : {bsig : BlockSig} -> (c : Code) -> Decidable (c.Okay fsigs bsigs ret bsig)
-    | bsig, stmt e c =>
-      let _ : Decidable (c.Okay fsigs bsigs ret bsig.bind) := instDecidable c
-      decidable_of_iff (e.Okay bsig.arity ∧ c.Okay fsigs bsigs ret bsig.bind)
-        ⟨λ ⟨a, b⟩ => Okay.stmt a b,
-         λ | (.stmt a b) => ⟨a, b⟩⟩
-    | bsig, trfr t => decidable_of_iff (t.Okay fsigs bsigs ret bsig)
-        ⟨Okay.trfr,
-         λ | Okay.trfr a => a⟩
-
-  -- instance instDecidableEq : DecidableEq Code
-  --   | stmt e c, stmt e' c' =>
-  --     let _ : Decidable (c = c') := instDecidableEq c c'
-  --     decidable_of_iff (e = e' ∧ c = c')
-  --     ⟨λ ⟨a, b⟩ => a ▸ b ▸ rfl,
-  --      λ p => ⟨congrArg (λ | stmt e c => e | _ => e) p,
-  --              congrArg (λ | stmt e c => c | _ => c) p⟩⟩
-  --   | trfr t, trfr t' => decidable_of_iff (t = t')
-  --       ⟨congrArg trfr,
-  --        congrArg (λ | trfr t => t | _ => t)⟩
-  --   | stmt _ _, trfr _ => isFalse (by simp)
-  --   | trfr _, stmt _ _ => isFalse (by simp)
   deriving instance DecidableEq for Code
 end Code
 
 namespace Block
-  variable
-    (fsigs : FuncSigs)
-    (bsigs : BlockSigs)
-    (ret : Nat)
+  @[simp] abbrev bsig | mk bsig _code => bsig
+  @[simp] abbrev code | mk _bsig code => code
 
-  abbrev bsig | mk bsig _code => bsig
-  abbrev code | mk _bsig code => code
+  inductive WF (fsigs bsigs ret) (b : Block) : Prop where
+    | mk (c : b.code.WF fsigs bsigs ret b.bsig)
 
-  inductive Okay (b : Block) : Prop where
-    | mk (c : b.code.Okay fsigs bsigs ret b.bsig)
+  namespace WF
+    instance (fsigs bsigs ret) : {b : Block} -> Decidable (b.WF fsigs bsigs ret)
+      | .mk bsig code =>
+        decidable_of_iff (code.WF fsigs bsigs ret bsig)
+          ⟨λ a => mk a, λ | mk a => a⟩
 
-  instance instDecidable : {b : Block} -> Decidable (b.Okay fsigs bsigs ret)
-    | mk bsig code =>
-      decidable_of_iff (code.Okay fsigs bsigs ret bsig)
-        ⟨λ a => .mk a, λ | .mk a => a⟩
+    theorem code {fsigs bsigs ret b} : WF fsigs bsigs ret b ->
+                 b.code.WF fsigs bsigs ret b.bsig
+      | .mk c => c
 
-  -- instance instDecidableEq : DecidableEq Block
-  --   | mk bsig code, mk bsig' code' =>
-  --     decidable_of_iff ((bsig, code) = (bsig', code'))
-  --       ⟨congrArg (λ (a, b) => mk a b),
-  --        λ x => congrArg (λ | .mk a b => (a, b)) x⟩
+    theorem weakening_bsigs
+            {fsigs bsigs bsigs' ret b} :
+            WF fsigs bsigs ret b ->
+            WF fsigs (bsigs ++ bsigs') ret b
+      | mk cwf => mk cwf.weakening_bsigs
+  end WF
 
   deriving instance DecidableEq for Block
 
-  instance instInhabited : Inhabited Block where
-    default := mk ⟨0, []⟩ (Code.trfr (Transfer.retn []))
+  instance : Inhabited Block where
+    default := mk ⟨0, []⟩ (.retn [])
 end Block
 
-inductive HeadIs {α β : Type} (l : List α) (m : α -> β) (b : β) : Prop where
-  | mk (h : m <$> l.head? = some b)
-
-namespace HeadIs
-  abbrev head?eq {α β : Type} {l : List α} {m : α -> β} {b : β} : HeadIs l m b -> m <$> l.head? = some b
-    | mk h => h
-
-  theorem nonnil {α β : Type} {l : List α} {m : α -> β} {b : β} (h : HeadIs l m b) : l ≠ [] :=
-    match (generalizing := true) l, h with
-      | a :: as, mk p => by simp
-
-  theorem headeq {α β : Type} {l : List α} {m : α -> β} {b : β} (h : HeadIs l m b) : m (l.head h.nonnil) = b :=
-    match (generalizing := true) l, h with
-      | _a :: _as, mk p => Option.some_inj.mp p
-
-  theorem head!eq {α β : Type} [Inhabited α] {l : List α}
-                  {m : α -> β} {b : β} (h : HeadIs l m b) :
-                  l.head h.nonnil = l.head! := by
-    cases l
-    · case nil => cases h; contradiction
-    · case cons => rfl
-
-  instance instDecidable {α β : Type} {m : α -> β} {b : β} [DecidableEq β] : {l : List α} -> Decidable (HeadIs l m b)
-    | l => decidable_of_iff (m <$> l.head? = some b) ⟨mk, λ | mk h => h⟩
-end HeadIs
-
 namespace Func
-  variable (fsigs : FuncSigs)
-  abbrev fsig | mk fsig _blocks => fsig
-  abbrev blocks | mk _fsig blocks => blocks
-  abbrev bsigs : Func -> BlockSigs | mk _fsig blocks => blocks.map (·.bsig)
+  @[simp] abbrev fsig | mk fsig _blocks => fsig
+  @[simp] abbrev blocks | mk _fsig blocks => blocks
+  @[simp] abbrev bsigs : Func -> BlockSigs | mk _fsig blocks => blocks.map (·.bsig)
+  @[simp] abbrev size | mk _fsig blocks => blocks.length
+  
+  @[simp] theorem size_eq_bsigs_length (f : Func) : f.bsigs.length = f.size :=
+    by simp
 
-  inductive Okay (f : Func) : Prop where
-    | mk (blocks : IVec (·.Okay fsigs (f.blocks.map (·.bsig)) f.fsig.ret) f.blocks)
+  inductive WF (fsigs : FuncSigs) (f : Func) : Prop where
+    | mk (blocks : IVec (·.WF fsigs (f.blocks.map (·.bsig)) f.fsig.ret) f.blocks)
          (head : HeadIs f.blocks (·.bsig) ⟨f.fsig.arity, []⟩)
 
-  instance instDecidable : {f : Func} -> Decidable (f.Okay fsigs)
-    | mk fsig blocks => decidable_of_iff
-        (IVec (·.Okay fsigs (blocks.map (·.bsig)) fsig.ret) blocks ∧
-         HeadIs blocks (·.bsig) ⟨fsig.arity, []⟩)
-        ⟨λ ⟨a, b⟩ => Okay.mk a b, λ | .mk a b => ⟨a, b⟩⟩
+  namespace WF
+    instance {fsigs : FuncSigs} : {f : Func} -> Decidable (f.WF fsigs)
+      | .mk fsig blocks => decidable_of_iff
+          (IVec (·.WF fsigs (blocks.map (·.bsig)) fsig.ret) blocks ∧
+           HeadIs blocks (·.bsig) ⟨fsig.arity, []⟩)
+          ⟨λ ⟨a, b⟩ => mk a b, λ | mk a b => ⟨a, b⟩⟩
 
-  -- instance instDecidableEq : DecidableEq Func
-  --   | mk fsig blocks, mk fsig' blocks' =>
-  --     decidable_of_iff ((fsig, blocks) = (fsig', blocks'))
-  --       ⟨congrArg (λ (a, b) => mk a b),
-  --        λ x => congrArg (λ | .mk a b => (a, b)) x⟩
+    theorem blocks {fsigs f} : WF fsigs f -> IVec (·.WF fsigs (f.blocks.map (·.bsig)) f.fsig.ret) f.blocks
+      | mk blocks _head => blocks
+    theorem head {fsigs f} : WF fsigs f -> HeadIs f.blocks (·.bsig) ⟨f.fsig.arity, []⟩
+      | mk _blocks head => head
+
+    theorem add_blocks
+            {fsigs fsig bs bs'} :
+            WF fsigs (.mk fsig bs) ->
+            IVec (·.WF fsigs ((bs ++ bs').map (·.bsig)) fsig.ret) bs' ->
+            WF fsigs (.mk fsig (bs ++ bs'))
+      | mk blocks head, bs'wf =>
+        mk (IVec.append (blocks.map
+             (λ b bwf => by simpa using bwf.weakening_bsigs)) bs'wf)
+           ⟨by rw[List.head?_eq_some_head,
+                  List.head_append_left head.nonnil,
+                  ← head.head?eq,
+                  List.head?_eq_head head.nonnil]⟩
+  end WF
+
   deriving instance DecidableEq for Func
 
-  instance instInhabited : Inhabited Func where
+  instance : Inhabited Func where
     default := mk ⟨0, 0⟩ default
+
+  instance : GetElem Func BlockIdx Block (λ f b => b < f.blocks.length) where
+    getElem f b p := f.blocks[b]
 end Func
 
 namespace Program
-  abbrev funs | mk funs => funs
-  abbrev fsigs : Program -> FuncSigs | mk funs => funs.map (·.fsig)
-  abbrev size | mk funs => funs.length
+  @[simp] abbrev funs | mk funs => funs
+  @[simp] abbrev fsigs : Program -> FuncSigs | mk funs => funs.map (·.fsig)
+  @[simp] abbrev size | mk funs => funs.length
 
-  theorem size_eq_fsigs_length (Pr : Program) : Pr.size = Pr.fsigs.length :=
+  @[simp] theorem size_eq_fsigs_length (P : Program) : P.fsigs.length = P.size :=
     by simp
 
-  inductive Okay (Pr : Program): Prop where
-    | mk (funcs : IVec (·.Okay Pr.fsigs) Pr.funs)
-         (head : HeadIs Pr.funs (·.fsig) ⟨0, 1⟩)
+  inductive WF (P : Program): Prop where
+    | mk (funcs : IVec (·.WF P.fsigs) P.funs)
+         (head : HeadIs P.funs (·.fsig) ⟨0, 1⟩)
 
-  instance instDecidable : {p : Program} -> Decidable p.Okay
-    | mk funs => decidable_of_iff
-        (IVec (·.Okay (funs.map (·.fsig))) funs ∧
-         HeadIs funs (·.fsig) ⟨0, 1⟩)
-        ⟨λ ⟨a, b⟩ => Okay.mk a b, λ | .mk a b => ⟨a, b⟩⟩
+  namespace WF
+    instance : {p : Program} -> Decidable p.WF
+      | .mk funs => decidable_of_iff
+          (IVec (·.WF (funs.map (·.fsig))) funs ∧
+           HeadIs funs (·.fsig) ⟨0, 1⟩)
+          ⟨λ ⟨a, b⟩ => mk a b, λ | mk a b => ⟨a, b⟩⟩
 
-  -- instance instDecidableEq : DecidableEq Program
-  --   | mk funs, mk funs' =>
-  --     decidable_of_iff (funs = funs')
-  --       ⟨congrArg mk, λ x => congrArg (λ | .mk a => a) x⟩
+    theorem funcs {P} : WF P -> IVec (·.WF P.fsigs) P.funs | .mk funcs _head => funcs
+    theorem head {P} : WF P -> HeadIs P.funs (·.fsig) ⟨0, 1⟩ | .mk _funcs head => head
+    theorem main_lt : {P : Program} -> WF P -> 0 < P.fsigs.length
+      | .mk (main :: funs), .mk funcs head => by simp
+    theorem main_lt' : {P : Program} -> WF P -> 0 < P.size
+      | .mk (main :: funs), .mk funcs head => by simp
+  end WF
+
   deriving instance DecidableEq for Program
+
+  instance : GetElem Program FuncIdx Func (λ P f => f < P.size) where
+    getElem P f p := P.funs[f]
+  
 end Program
 
