SporkProofs/HeadIs.lean
@@ -1,0 +1,46 @@
+inductive HeadIs {α β : Type} (l : List α) (m : α -> β) (b : β) : Prop where
+  | mk (h : m <$> l.head? = some b)
+
+namespace HeadIs
+  abbrev head?eq {α β : Type} {l : List α} {m : α -> β} {b : β} : HeadIs l m b -> m <$> l.head? = some b
+    | mk h => h
+
+  theorem nonnil {α β : Type} {l : List α} {m : α -> β} {b : β} (h : HeadIs l m b) : l ≠ [] :=
+    match (generalizing := true) l, h with
+      | a :: as, mk p => by simp
+
+  theorem headeq {α β : Type} {l : List α} {m : α -> β} {b : β} (h : HeadIs l m b) : m (l.head h.nonnil) = b :=
+    match (generalizing := true) l, h with
+      | _a :: _as, mk p => Option.some_inj.mp p
+
+  theorem head!eq {α β : Type} [Inhabited α] {l : List α}
+                  {m : α -> β} {b : β} (h : HeadIs l m b) :
+                  l.head h.nonnil = l.head! := by
+    cases l
+    · case nil => nomatch h
+    · case cons => rfl
+
+  theorem zero_lt {α β : Type} : {l : List α} -> {m : α -> β} -> {b : β} -> (h : HeadIs l m b) -> 0 < l.length
+    | _ :: _, _, _, _ => by simp    
+
+  theorem get0eq {α β : Type} {l : List α} {m : α -> β} {b : β} (h : HeadIs l m b) : m (l[0]'h.zero_lt) = b :=
+    List.head_eq_getElem h.nonnil ▸ headeq h
+
+  theorem headtail {α β : Type} {l : List α} {m : α -> β} {b : β} (h : HeadIs l m b) : l = l.head h.nonnil :: l.tail :=
+    by cases l
+       · case nil => nomatch h
+       · case cons => rfl
+
+  theorem map_head {α β : Type} {l : List α} {m : α -> β} {b : β} (h : HeadIs l m b) : (l.map m).head? = some b :=
+    by cases l
+       · case nil => nomatch h
+       · case cons => exact h.head?eq
+
+  theorem append {α β : Type} {l₁ l₂ : List α} {m : α -> β} {b : β} (h : HeadIs l₁ m b) : HeadIs (l₁ ++ l₂) m b :=
+    by cases l₁
+       · case nil => nomatch h
+       · case cons => apply mk; simpa using h.headeq
+
+  instance instDecidable {α β : Type} {m : α -> β} {b : β} [DecidableEq β] : {l : List α} -> Decidable (HeadIs l m b)
+    | l => decidable_of_iff (m <$> l.head? = some b) ⟨mk, λ | mk h => h⟩
+end HeadIs
