SporkProofs/Inline.lean
@@ -1,0 +1,277 @@
+import SporkProofs.Syntax
+import SporkProofs.Semantics
+
+structure Extra where
+  offset : Nat
+  bsig : BlockSig
+
+@[simp] def inlinedArgs (extra : Extra) (scope : Nat) (args : List Var) : List Var :=
+  args ++ (List.range' scope extra.bsig.arity).map Var.mk
+
+@[simp] def inlinedCont (extra : Extra) (scope : Nat) : Cont -> Cont
+  | .mk b args => .mk (b + extra.offset) (inlinedArgs extra scope args)
+
+@[simp] def inlinedCode (bret : BlockIdx) (extra : Extra) (scope : Nat) : Code -> Code
+  | .stmt e c =>
+    .stmt e (inlinedCode bret extra scope.succ c)
+  | .goto bnext =>
+    .goto (inlinedCont extra scope bnext)
+  | .ite cond bthen belse =>
+    .ite cond
+         (inlinedCont extra scope bthen)
+         (inlinedCont extra scope belse)
+  | .call h args bret =>
+    .call h args (inlinedCont extra scope bret)
+  | .retn args =>
+    .goto (.mk bret (inlinedArgs extra scope args))
+  | .spork bbody hspwn args =>
+    .spork (inlinedCont extra scope bbody) hspwn args
+  | .spoin bunpr bprom =>
+    .spoin (inlinedCont extra scope bunpr)
+           (inlinedCont extra scope bprom)
+
+@[simp] def inlinedBlock (bret : BlockIdx) (extra : Extra) (b : Block) : Block :=
+  Block.mk (b.bsig + extra.bsig) (inlinedCode bret extra b.bsig.arity b.code)
+
+theorem inlinedArgsRangeWF :
+    (extraArity : Nat) -> (scope : Nat) ->
+    IVec (·.WF (scope + extraArity)) ((List.range' scope extraArity).map Var.mk)
+  | 0, scope => .nil
+  | .succ extraArity, scope =>
+    .cons (.mk (by simp))
+          (Nat.add_succ scope extraArity ▸
+           Nat.succ_add scope extraArity ▸
+           inlinedArgsRangeWF extraArity scope.succ)
+
+theorem inlinedArgsWF' (extra : Extra) {scope : Nat} : {args : List Var} ->
+                       IVec (·.WF scope) args -> IVec (·.WF (scope + extra.bsig.arity)) args
+  | [], .nil => .nil
+  | _a :: _args, .cons awf argswf =>
+    .cons (Var.WF.mk (Nat.lt_add_right extra.bsig.arity awf.idx))
+          (inlinedArgsWF' extra argswf)
+
+theorem inlinedArgsWF (extra : Extra) {scope : Nat} {args : List Var}
+                      (wf : IVec (·.WF scope) args) :
+                      IVec (·.WF (scope + extra.bsig.arity)) (inlinedArgs extra scope args) :=
+  (inlinedArgsWF' extra wf).append (inlinedArgsRangeWF extra.bsig.arity scope)
+
+theorem inlinedContWFRets
+        {bsigs bsigs' bsig rets} (extra : Extra) {c : Cont}
+        (bslen : bsigs.length = extra.offset)
+        (wf : c.WFRets bsigs' bsig rets) :
+        (inlinedCont extra bsig.arity c).WFRets
+          (bsigs ++ bsigs'.map (· + extra.bsig)) (bsig + extra.bsig) rets :=
+  .mk (by simp[← bslen, Nat.add_comm c.b bsigs.length, wf.blt])
+      (by simp[wf.bsig, Nat.add_comm c.b extra.offset, ← bslen]
+          show BlockSig.mk (c.args.length + rets + extra.bsig.arity)
+                           (bsig.sporkNest ++ extra.bsig.sporkNest) =
+               BlockSig.mk (c.args.length + extra.bsig.arity + rets)
+                           (bsig.sporkNest ++ extra.bsig.sporkNest)
+          rw[Nat.add_assoc, Nat.add_comm rets extra.bsig.arity, ← Nat.add_assoc])
+      (inlinedArgsWF extra wf.args)
+
+theorem inlinedContWF
+        {bsigs bsigs' bsig} (extra : Extra) {c : Cont}
+        (bslen : bsigs.length = extra.offset)
+        (wf : c.WF bsigs' bsig) :
+        (inlinedCont extra bsig.arity c).WF
+          (bsigs ++ bsigs'.map (· + extra.bsig)) (bsig + extra.bsig) :=
+  (inlinedContWFRets extra bslen wf.cast0).cast0
+
+theorem inlinedAtomWF {Γ : Nat} (extraArity : Nat) : {a : Atom} -> a.WF Γ -> a.WF (Γ + extraArity)
+  | .val _v, _wf => .val
+  | .var _v, wf => .var (.mk (Nat.lt_add_right extraArity wf.vwf.idx))
+
+theorem inlinedExprWF {Γ : Nat} (extraArity : Nat) : {e : Expr} -> e.WF Γ -> e.WF (Γ + extraArity)
+  | .nop _a, .nop awf =>
+    .nop (inlinedAtomWF extraArity awf)
+  | .uop _o _a, .uop awf =>
+    .uop (inlinedAtomWF extraArity awf)
+  | .bop _o _a _b, .bop awf bwf =>
+    .bop (inlinedAtomWF extraArity awf) (inlinedAtomWF extraArity bwf)
+
+theorem inlinedCodeWF
+    {fsigs bsigs bsigs' ret ret' bsig bret}
+    (bretlt : bret < bsigs.length)
+    (extra : Extra)
+    (bretsig : bsigs[bret] = ⟨ret + extra.bsig.arity, extra.bsig.sporkNest⟩)
+    (bslen : bsigs.length = extra.offset) :
+    {c : Code} ->
+    c.WF fsigs bsigs' ret bsig ->
+    (inlinedCode bret extra bsig.arity c).WF
+      fsigs (bsigs ++ bsigs'.map (· + extra.bsig)) ret' (bsig + extra.bsig)
+  | .stmt e c, wf =>
+    .stmt (inlinedExprWF extra.bsig.arity wf.stmt_expr)
+          (by simpa[Nat.add_right_comm bsig.arity extra.bsig.arity 1]
+              using inlinedCodeWF (bsig := bsig.bind) bretlt extra bretsig bslen (wf.stmt_code))
+  | .goto bnext, wf =>
+    .goto (inlinedContWF extra bslen wf.goto_bnext)
+  | .ite cond bthen belse, wf =>
+    .ite (inlinedAtomWF extra.bsig.arity wf.ite_cond)
+         (inlinedContWF extra bslen wf.ite_bthen)
+         (inlinedContWF extra bslen wf.ite_belse)
+  | .call h args bret', wf =>
+    .call wf.call_flt
+          (wf.call_arity)
+          (inlinedArgsWF' extra wf.call_args)
+          (inlinedContWFRets extra bslen wf.call_bret)
+  | .retn args, .retn sn_nil len argswf =>
+    let x : bret < (bsigs ++ bsigs').length :=
+      by simp[Nat.lt_add_right bsigs'.length bretlt]
+    .goto (.mk (by simp[Nat.lt_add_right bsigs'.length bretlt])
+               (by simp[← len]
+                   rw[List.getElem_append_left (bs := bsigs'.map (· + extra.bsig)) bretlt]
+                   simp[sn_nil, bretsig])
+               (inlinedArgsWF extra argswf))
+  | .spork bbody hspwn args, wf =>
+    .spork wf.spork_flt
+           wf.spork_arity
+           (inlinedArgsWF' extra wf.spork_args)
+           (inlinedContWF extra bslen wf.spork_bbody)
+  | .spoin bunpr bprom, wf =>
+    .spoin (by simp[wf.spoin_sn_nonnil])
+           (by simp[List.tail_append_of_ne_nil wf.spoin_sn_nonnil]
+               exact inlinedContWF extra bslen wf.spoin_bunpr)
+           (by simp[List.tail_append_of_ne_nil wf.spoin_sn_nonnil,
+                    List.head_append_left wf.spoin_sn_nonnil]
+               exact inlinedContWFRets extra bslen wf.spoin_bprom)
+
+theorem inlinedBlockWF
+    {fsigs bsigs bsigs' ret ret' bret}
+    (bretlt : bret < bsigs.length)
+    (extra : Extra)
+    (bretsig : bsigs[bret] = ⟨ret + extra.bsig.arity, extra.bsig.sporkNest⟩)
+    (bslen : bsigs.length = extra.offset)
+    {b : Block}
+    (wf : b.WF fsigs bsigs' ret) :
+    (inlinedBlock bret extra b).WF
+      fsigs (bsigs ++ bsigs'.map (· + extra.bsig)) ret' :=
+  .mk (inlinedCodeWF bretlt extra bretsig bslen wf.1)
+
+@[simp] def inlinedFuncBody (g : Func) (bret : Cont) (sporks : SporkSig) (offset : Nat) : List Block :=
+  g.blocks.map (inlinedBlock bret.b (.mk offset (.mk bret.args.length sporks)))
+
+theorem inlinedFuncBodyWF
+          {fsigs bsigs ret g bret sporks}
+          (bretlt : bret.b < bsigs.length)
+          (bretsig : bsigs[bret.b] = ⟨g.fsig.ret + bret.args.length, sporks⟩)
+          (wf : g.WF fsigs) :
+          IVec (·.WF fsigs (bsigs ++ List.map (· + .mk bret.args.length sporks) g.bsigs) ret)
+               (inlinedFuncBody g bret sporks bsigs.length) :=
+  wf.blocks.from_map'
+    (inlinedBlock bret.b (.mk bsigs.length (.mk bret.args.length sporks)))
+    (λ _b => inlinedBlockWF bretlt (.mk bsigs.length (.mk bret.args.length sporks)) bretsig rfl)
+
+@[simp] def replaceCallInCode (g : FuncIdx) (offset : Nat) (c : Code) : Option (Code × Cont) :=
+  let (e, ⟨t, _p⟩) := c.split
+  match t with
+    | .call h args bret =>
+      if h = g then
+        some (Code.join e (Code.goto (.mk offset (args ++ bret.args))), bret)
+      else
+        none
+    | _ => none
+
+
+@[simp] def inlinedFuncH (g : Func) (gidx : FuncIdx) :
+                 List Block -> List Block -> List Block -> List Block
+  | bacc, [], gacc => bacc ++ gacc
+  | bacc, .mk bsig c :: bs, gacc =>
+    let (b', gacc') :=
+      (replaceCallInCode gidx
+          (bacc ++ [Block.mk bsig c] ++ bs ++ gacc).length c).elim
+        (.mk bsig c, [])
+        (λ (c', bret) =>
+          (.mk bsig c',
+           inlinedFuncBody g bret bsig.sporkNest
+             (bacc ++ [Block.mk bsig c'] ++ bs ++ gacc).length))
+    inlinedFuncH g gidx (bacc ++ [b']) bs (gacc ++ gacc')
+
+theorem inlinedFuncHWF
+        {fsigs fsig g gidx bacc gacc} :
+        {bs : List Block} ->
+        g.WF fsigs ->
+        (_ : gidx < fsigs.length) ->
+        fsigs[gidx] = g.fsig ->
+        (Func.mk fsig (bacc ++ bs ++ gacc)).WF fsigs ->
+        (Func.mk fsig (inlinedFuncH g gidx bacc bs gacc)).WF fsigs
+  | [], gwf, glt, gsig, wf => List.append_nil bacc ▸ wf
+  | .mk bsig c :: bs, gwf, glt, gsig, wf => by
+    simp
+    match cspliteq : c.split with
+      | (es, ⟨t, t_neq_stmt⟩) =>
+        cases t <;> simp <;> try (apply inlinedFuncHWF gwf glt gsig; simpa using wf)
+        · case call h args bret =>
+          if heqg : h ≠ gidx then
+            simp[heqg]
+            apply inlinedFuncHWF gwf glt gsig
+            simpa using wf
+          else
+            let heqg := Decidable.of_not_not heqg
+            rw[heqg]
+            simp[heqg] at cspliteq
+            simp
+            let c' : Code :=
+              .join es (.goto (.mk (bacc.length + (bs.length + gacc.length + 1))
+                                   (args ++ bret.args)))
+            let gacc' := inlinedFuncBody g bret bsig.sporkNest
+                           (bacc ++ [Block.mk bsig c'] ++ bs ++ gacc).length
+            let bsigs := (bacc ++ Block.mk bsig c' :: bs ++ gacc ++ gacc').map (·.bsig)
+            let wf' := wf.blocks.get ⟨bacc.length, by simp⟩
+            simp at wf'
+            let cwf := wf'.code
+            let splitwf := Code.WF.split_wf cwf
+            simp[cspliteq] at splitwf
+            let c'wf : c'.WF fsigs bsigs fsig.ret bsig := by
+              simp[c', bsigs]
+              apply Code.WF.join_wf
+              · exact λ ⟨i, il⟩ => splitwf.1 ⟨i, by simp_all⟩
+              · apply Code.WF.goto; apply Cont.WF.mk <;> simp
+                · simp[gacc']
+                  let gh := gwf.head.get0eq
+                  simp at gh; rw[gh]; simp
+                  show g.fsig.arity = args.length
+                  exact gsig ▸ splitwf.2.call_arity
+                · exact splitwf.2.call_args.append splitwf.2.call_bret.args
+                · match gacc'eq : gacc' with
+                    | [] => simp[gacc'] at gacc'eq
+                            let ghead := gwf.head.headtail
+                            simp[gacc'eq] at ghead
+                    | _ :: _ => simp
+            let b'wf : (Block.mk bsig c').WF fsigs bsigs fsig.ret := .mk c'wf
+            let wfblocks := wf.blocks
+            let ⟨tmp, gaccwf⟩ := wf.blocks.unappend
+            let ⟨baccwf, tmp'⟩ := tmp.unappend
+            let bswf := tmp'.tail
+            let helper {l : List Block} (v : IVec (Block.WF fsigs (List.map (fun x => x.bsig) (Func.mk fsig (bacc ++ Block.mk bsig c :: bs ++ gacc)).blocks) (Func.mk fsig (bacc ++ Block.mk bsig c :: bs ++ gacc)).fsig.ret) l) : IVec (Block.WF fsigs (List.map (fun x => x.bsig) (Func.mk fsig (bacc ++ [Block.mk bsig c'] ++ bs ++ (gacc ++ gacc'))).blocks) (Func.mk fsig (bacc ++ [Block.mk bsig c'] ++ bs ++ (gacc ++ gacc'))).fsig.ret) l :=
+              v.map (λ b x => by simpa using x.weakening_bsigs (bsigs' := gacc'.map (·.bsig)))
+            let wf'' : Func.WF fsigs (.mk fsig (bacc ++ [.mk bsig c'] ++ bs
+                                                  ++ (gacc ++ gacc'))) := by
+              apply Func.WF.mk
+              · apply IVec.append
+                · apply IVec.append
+                  · apply IVec.append
+                    · exact helper baccwf
+                    · apply IVec.singleton
+                      simpa[bsigs] using b'wf
+                  · exact helper bswf
+                · apply IVec.append
+                  · exact helper gaccwf
+                  · simp[gacc']; let x := @inlinedFuncBodyWF fsigs ((bacc ++ [Block.mk bsig c'] ++ bs ++ gacc).map (·.bsig)) fsig.ret g bret bsig.sporkNest (by simpa using splitwf.2.call_bret.blt) (by simpa[gsig, Nat.add_comm] using splitwf.2.call_bret.bsig) gwf; simp at x; exact x
+              · cases bacc <;> simp <;> simp at wf <;>
+                apply HeadIs.mk <;> simpa using wf.head.get0eq
+            simpa[c', gacc']
+            using @inlinedFuncHWF fsigs fsig g gidx (gacc ++ gacc') bs
+                                  gwf glt gsig (bacc := bacc ++ [.mk bsig c']) wf''
+
+/--
+Inline each call to g in the body of f
+-/
+def inlinedFunc (f g : Func) (gidx : FuncIdx) : Func :=
+  .mk f.fsig (inlinedFuncH g gidx [] f.blocks [])
+
+theorem inlinedFuncWF {fsigs} {f g : Func} {gidx : FuncIdx}
+                      (gwf : g.WF fsigs) (glt : gidx < fsigs.length)
+                      (gsig : fsigs[gidx] = g.fsig) (wf : f.WF fsigs) :
+                      (inlinedFunc f g gidx).WF fsigs :=
+  inlinedFuncHWF gwf glt gsig ((List.append_nil f.blocks).symm ▸ wf)
