SporkProofs/Preservation.lean
@@ -3,234 +3,183 @@ import SporkProofs.Semantics
 
 namespace Step
   theorem preserve_retjoin_stack_cons
-    {Pr K f ρ ρ' X X' c c'} :
-      CallStack.retjoin Pr (K ⬝ ⟨f, ρ, X, c⟩) =
-        CallStack.retjoin Pr (K ⬝ ⟨f, ρ', X', c'⟩)
+    {P K f ρ₁ ρ₂ X₁ X₂ c₁ c₂} :
+      CallStack.retjoin P (K ⬝ ⟨f, ρ₁, X₁, c₁⟩) =
+      CallStack.retjoin P (K ⬝ ⟨f, ρ₂, X₂, c₂⟩)
     := by cases K <;> rfl
 
-  theorem preserve_retjoin_stack_cons_cons {Pr K k k'} :
-      (K ⬝ k ⬝ k').retjoin Pr = (K ⬝ k).retjoin Pr :=
+  @[simp] theorem preserve_retjoin_stack_cons_cons {P K k k'} :
+      (K ⬝ k ⬝ k').retjoin P = (K ⬝ k).retjoin P :=
     by cases K <;> rfl
 
-  theorem preserve_retjoin_stack_cons_nonnil {Pr K k} :
-      K ≠ ∅ → (K ⬝ k).retjoin Pr = K.retjoin Pr := by
+  @[simp] theorem preserve_retjoin_stack_cons_nonnil {P K k} :
+      K ≠ ∅ → (K ⬝ k).retjoin P = K.retjoin P := by
     cases K <;> intro nn
     · case nil => contradiction
     · case cons => rfl
 
-  -- List.append_ne_nil_of_left_ne_nil
   theorem stack_append_left_nonnil : (s t : CallStack) -> (h : s ≠ ∅) -> s ++ t ≠ ∅
     | s, .nil, h => h
     | s, K ⬝ k, h => by simp
 
-  theorem preserve_retjoin_stack_append {Pr K k} : {K' : CallStack} ->
-      CallStack.retjoin Pr (K ⬝ k ++ K') = CallStack.retjoin Pr (K ⬝ k)
+  @[simp] theorem preserve_retjoin_stack_append {P K k} : {K' : CallStack} ->
+      CallStack.retjoin P (K ⬝ k ++ K') = CallStack.retjoin P (K ⬝ k)
     | .nil => rfl
     | K' ⬝ k' => preserve_retjoin_stack_cons_nonnil
                    (stack_append_left_nonnil (K ⬝ k) K' (by simp)) ▸
                  preserve_retjoin_stack_append (K' := K')
 
-  theorem preserve_retjoin {Pr : Program} : {P P' : ThreadPool} ->
-                         Pr ⊢ P ↦ P' -> {ρ : SporkSig} -> P.Okay Pr ρ ->
-                         P.retjoin Pr = P'.retjoin Pr
-  | P, P', s => by
-    cases s <;> intro Pₒₖ <;>
+  theorem preserve_retjoin {P : Program} : {R R' : ThreadTree} ->
+                         P ⊢ R ↦ R' -> R.WF P ->
+                         R.retjoin P = R'.retjoin P
+  | R, R', s => by
+    cases s <;> intro Rwf <;>
     try (exact preserve_retjoin_stack_cons)
-    · case stepₗ P P' P₂ s =>
-        simp_all!; match Pₒₖ with
-          | .cat Pok P2ok => exact preserve_retjoin s Pok
-    · case stepᵣ P₁ P P' s =>
+    · case congr_parent Rp Rp' Rc s =>
+        simp only [ThreadTree.retjoin]; match Rwf with
+          | .node Rpwf Rcwf Rpp Rcp => exact preserve_retjoin s Rpwf
+    · case congr_child Rp Rc Rc' s =>
         rfl
     · case retn f g K ρ' X Y y bret =>
         exact preserve_retjoin_stack_cons (K := K)
     · case promote f unpr g prom X K c K' u p =>
-        simp[ThreadPool.retjoin];
-        rw[preserve_retjoin_stack_append,
-           preserve_retjoin_stack_append,
-           preserve_retjoin_stack_cons]
+        simp; rw[preserve_retjoin_stack_cons]
 
-  theorem goto_okay_rets
-      {Pr} (Prok : Pr.Okay) {f canProm ρ} {X Y : ValMap} {bnext} {y : List Var}
-      (p : f < Pr.size)
-      (ρok : ρ.Okay Pr.fsigs canProm)
-      (bnext_ok : bnext.OkayRets Pr.funs[f].bsigs ⟨X.length, ρ.sig⟩ y.length)
-      (y_ok : IVec (·.Okay Y.length) y) :
-      StackFrame.Okay Pr none canProm
-        ⟨f, ρ, X[bnext.args]! ++ Y[y]!, codeOf Pr f bnext⟩ :=
-    let ⟨bok, sigok, x_ok⟩ := bnext_ok
-    let bok' : bnext.b < Pr.funs[f].blocks.length :=
-      List.length_map Block.bsig ▸ bok
-    let xlen : bnext.args.length = X[bnext.args].length :=
-      x_ok.map_length (λ x xₒₖ => X[x])
-    let ylen : y.length = Y[y].length :=
-      y_ok.map_length (λ y yₒₖ => Y[y])
-    let code_ok : Pr.funs[f]!.blocks[bnext.b]!.code.Okay
-                    Pr.fsigs Pr.funs[f].bsigs Pr.funs[f].fsig.ret
-                    ⟨(X[bnext.args]! ++ Y[y]!).length, ρ.sig⟩ := by
-      rw[codeOfGetElem p bok',
-         argsOfGetElem x_ok,
-         argsOfGetElem y_ok,
-         List.length_append,
-         ← xlen, ← ylen, ← sigok]
-      simp; exact ((Prok.1.get ⟨f, p⟩).1.get ⟨bnext.b, bok'⟩).1
-    ⟨p, ρok, rfl, .code code_ok⟩
+  theorem preserve_prom {P : Program} : {R R' : ThreadTree} ->
+                         P ⊢ R ↦ R' -> R.WF P -> R.prom = R'.prom
+  | R, R', s => by
+    cases s <;> intro Rwf <;> try simp
+    · case congr_parent Rp Rp' Rc Rp_Rp' =>
+      rw[preserve_prom Rp_Rp' Rwf.parent]
+    · case promote f unpr g prom X K c K' u p =>
+      simp[p]
 
-  theorem goto_okay
-      {Pr} (Prok : Pr.Okay) {f canProm ρ} {X : ValMap} {bnext}
-      (p : f < Pr.size)
-      (ρok : ρ.Okay Pr.fsigs canProm)
-      (bnext_ok : bnext.Okay Pr.funs[f].bsigs ⟨X.length, ρ.sig⟩) :
-      StackFrame.Okay Pr none canProm ⟨f, ρ, X[bnext.args]!, codeOf Pr f bnext⟩ :=
-    List.append_nil X[bnext.args]! ▸
-    goto_okay_rets Prok (Y := []) (y := []) p ρok bnext_ok.cast0 .nil
-
-  theorem entry_okay
-      {Pr} (Prok : Pr.Okay) {f canProm} {X : List Val}
-      (p : f < Pr.size)
-      (sigok : Pr.funs[f].fsig.arity = X.length) :
-      StackFrame.Okay Pr none canProm ⟨f, ∅, X, codeEntry Pr f⟩ :=
-    let fok := Prok.1.get ⟨f, p⟩
-    let c' : Code.Okay Pr.fsigs Pr.funs[f].bsigs Pr.funs[f].fsig.ret
-              ⟨X.length, []⟩
-              Pr.funs[f]!.blocks.head!.code :=
-      sigok ▸
-      Eq.symm (getElem!_pos Pr.funs f p) ▸
-      fok.2.headeq ▸
-      fok.2.head!eq ▸
-      (fok.1.head fok.2.nonnil).1
-    ⟨p, SpawnDeque.empty_okay, rfl, .code c'⟩
-
-  theorem goto_entry_okay
-      {Pr} (Prok : Pr.Okay) {f canProm} {X : ValMap} {x : List Var}
-      (p : f < Pr.size)
-      (xok : IVec (·.Okay X.length) x)
-      (sigok : Pr.funs[f].fsig.arity = x.length) :
-      StackFrame.Okay Pr none canProm ⟨f, ∅, X[x]!, codeEntry Pr f⟩ :=
-    entry_okay Prok p (argsOfGetElem xok ▸
-                       xok.map_length (λ x xₒₖ => X[x]) ▸
-                       sigok)
   
-  open ThreadPool.Okay (leaf cat) in
-  theorem preservation {Pr : Program} (Prok : Pr.Okay) :
-                       {P P' : ThreadPool} -> {ρ : SporkSig} ->
-                       P.Okay Pr ρ -> Pr ⊢ P ↦ P' -> P'.Okay Pr ρ := by
-    intro P P' ρ ok P_P'; cases P_P' <;> cases ok
+  open ThreadTree.WF (thread node) in
+  theorem preservation {P : Program} (Pwf : P.WF) :
+                       {R R' : ThreadTree} ->
+                       R.WF P -> P ⊢ R ↦ R' -> R'.WF P := by
+    intro R R' wf R_R'; cases R_R' <;> cases wf
 
-    · case stepₗ P P' P₂ P_P' P2ok Pok =>
-        exact cat (preservation Prok Pok P_P') P2ok
+    · case congr_parent Rp Rp' Rc Rp_Rp' Rpwf Rcwf Rcp Rpp =>
+        exact node (preservation Pwf Rpwf Rp_Rp') Rcwf (preserve_prom Rp_Rp' Rpwf ▸ Rpp) Rcp
 
-    · case stepᵣ P₁ P P' P_P' Pok P1ok =>
-        exact cat (preserve_retjoin P_P' Pok ▸ P1ok) (preservation Prok Pok P_P')
+    · case congr_child Rp Rc Rc' Rc_Rc' Rpwf Rcwf Rcp Rpp =>
+        exact node Rpwf (preservation Pwf Rcwf Rc_Rc')
+                        (preserve_retjoin Rc_Rc' Rcwf ▸ Rpp)
+                        (preserve_prom Rc_Rc' Rcwf ▸ Rcp)
 
-    · case stmt f K ρ X e v c a ok =>
-        apply @leaf Pr (K ⬝ ⟨f, ρ, X.concat v, .code c⟩)
-        exact match ok with
-           | Kok ⬝ₒₖ (.mk p ρok _ (.code (.stmt eok cok))) =>
-             Kok ⬝ₒₖ (.mk p ρok rfl (.code
-                 (by simp[BlockSig.bind] at cok; simp; exact cok)))
+    · case stmt f K ρ X e v c a wf =>
+        apply thread
+        exact match wf with
+           | Kwf ⬝wf (.mk p ρwf _ (.code (.stmt ewf cwf))) =>
+             Kwf ⬝wf (.mk p ρwf rfl (.code
+                 (by simp[BlockSig.bind] at cwf; simp; exact cwf)))
 
-    · case goto f K ρ X bnext ok =>
-        apply @leaf Pr (K ⬝ ⟨f, ρ, X[bnext.args]!, codeOf Pr f bnext⟩)
-        exact match ok with
-          | Kok ⬝ₒₖ (.mk p ρok _ (.code (.trfr (.goto bnext_ok))))=>
-            Kok ⬝ₒₖ (goto_okay Prok p ρok bnext_ok)
+    · case goto f K ρ X bnext wf =>
+        apply thread
+        exact match wf with
+          | Kwf ⬝wf (.mk p ρwf _ (.code (.goto bnext_wf)))=>
+            Kwf ⬝wf (.goto Pwf p ρwf bnext_wf)
 
-    · case ite_true f K ρ X cond bthen belse n cond_n neq0 ok =>
-        apply @leaf Pr (K ⬝ ⟨f, ρ, X[bthen.args]!, codeOf Pr f bthen⟩)
-        exact match ok with
-          | Kok ⬝ₒₖ (.mk p ρok _ (.code (.trfr (.ite cond_ok bthen_ok belse_ok)))) =>
-            Kok ⬝ₒₖ (goto_okay Prok p ρok bthen_ok)
+    · case ite_true f K ρ X cond bthen belse n cond_n neq0 wf =>
+        apply thread
+        exact match wf with
+          | Kwf ⬝wf (.mk p ρwf _ (.code (.ite cond_wf bthen_wf belse_wf))) =>
+            Kwf ⬝wf (.goto Pwf p ρwf bthen_wf)
 
-    · case ite_false f K ρ X cond bthen belse cond_0 ok =>
-        apply @leaf Pr (K ⬝ ⟨f, ρ, X[belse.args]!, codeOf Pr f belse⟩)
-        exact match ok with
-          | Kok ⬝ₒₖ (.mk p ρok _ (.code (.trfr (.ite cond_ok bthen_ok belse_ok)))) =>
-            Kok ⬝ₒₖ (goto_okay Prok p ρok belse_ok)
+    · case ite_false f K ρ X cond bthen belse cond_0 wf =>
+        apply thread
+        exact match wf with
+          | Kwf ⬝wf (.mk p ρwf _ (.code (.ite cond_wf bthen_wf belse_wf))) =>
+            Kwf ⬝wf (.goto Pwf p ρwf belse_wf)
 
-    · case call f g K ρ X x bret ok =>
-        apply @leaf Pr (K ⬝ ⟨f, ρ, X, .cont bret⟩ ⬝ ⟨g, ∅, X[x]!, codeEntry Pr g⟩)
-        exact match ok with
-          | Kok ⬝ₒₖ kok@(.mk fok ρok _ (.code (.trfr (.call flt sigok x_ok
-                bret_ok@(.mk bret_lt bret_sig_okay argsok))))) =>
-              let bret_ok' : Cont.OkayRets Pr.funs[f].bsigs ⟨X.length, ρ.sig⟩
-                               Pr.fsigs[g].ret bret :=
-                Pr.funs.getElem_map (·.fsig) ▸ bret_ok
-              let gframe_ok :=
-                goto_entry_okay (f := g) Prok (Pr.size_eq_fsigs_length ▸ flt) x_ok
-                  (Pr.funs.getElem_map (·.fsig) ▸ sigok)
-              let glt := gframe_ok.flt
-              let bret_ok'' : Cont.OkayRets Pr.funs[f].bsigs ⟨X.length, ρ.sig⟩
-                                Pr.funs[g].fsig.ret bret :=
-                Pr.funs.getElem_map (·.fsig) ▸ bret_ok'
-              Kok ⬝ₒₖ ⟨fok, ρok, rfl, .cont bret_ok''⟩ ⬝ₒₖ gframe_ok
+    · case call f g K ρ X x bret wf =>
+        apply thread
+        exact match wf with
+          | Kwf ⬝wf kwf@(.mk fwf ρwf _ (.code (.call flt sigwf x_wf
+                bret_wf@(.mk bret_lt bret_sig_wf argswf)))) =>
+              let bret_wf' : Cont.WFRets P[f].bsigs ⟨X.length, ρ.sig⟩
+                               P.fsigs[g].ret bret :=
+                P.funs.getElem_map (·.fsig) ▸ bret_wf
+              let gframe_wf :=
+                StackFrame.WF.goto_entry
+                  (f := g) Pwf (P.size_eq_fsigs_length ▸ flt)
+                  x_wf (P.funs.getElem_map (·.fsig) ▸ sigwf)
+              let glt := gframe_wf.flt
+              let bret_wf'' : Cont.WFRets P[f].bsigs ⟨X.length, ρ.sig⟩
+                                P[g].fsig.ret bret :=
+                P.funs.getElem_map (·.fsig) ▸ bret_wf'
+              Kwf ⬝wf ⟨fwf, ρwf, rfl, .cont bret_wf''⟩ ⬝wf gframe_wf
 
-    · case retn f g K ρ X Y y bret ok =>
-        apply @leaf Pr (K ⬝ ⟨f, ρ, X[bret.args]! ++ Y[y]!, codeOf Pr f bret⟩)
-        exact match ok with
-          | Kok ⬝ₒₖ (.mk flt ρok _ (.cont bret_ok))
-                ⬝ₒₖ (.mk glt ⟨.nil, _⟩ _ (.code (.trfr (.retn _ ylen y_ok)))) =>
-            Kok ⬝ₒₖ (goto_okay_rets Prok flt ρok (ylen ▸ bret_ok) y_ok)
+    · case retn f g K ρ X Y y bret wf =>
+        apply thread
+        exact match wf with
+          | Kwf ⬝wf (.mk flt ρwf _ (.cont bret_wf))
+                ⬝wf (.mk glt ⟨.nil, _⟩ _ (.code (.retn _ ylen y_wf))) =>
+            Kwf ⬝wf (.goto_rets Pwf flt ρwf (ylen ▸ bret_wf) y_wf)
 
-    · case spork f K ρ X g g_args bbody ok =>
-       apply @leaf Pr (K ⬝ ⟨f, ρ.push ⟨g, X[g_args]!, Pr.funs[g]!.fsig.ret⟩,
-                            X[bbody.args]!, codeOf Pr f bbody⟩)
-       exact match ok with
-         | Kok ⬝ₒₖ ⟨flt, ⟨unpr_ok, prom_ok⟩, _, .code
-               (.trfr (.spork glt gsig g_args_ok bbody_ok))⟩ =>
-           let glt' : g < Pr.funs.length := List.length_map (α := Func) (·.fsig) ▸ glt
-           let h : FuncSig.mk X[g_args]!.length Pr.funs[g]!.fsig.ret = Pr.fsigs[g] :=
-             argsOfGetElem g_args_ok ▸
-             getElem!_pos Pr.funs g glt' ▸
-             congrArg₂ FuncSig.mk
-               (g_args_ok.map_length (λ x xₒₖ => X[x]) ▸ Eq.symm gsig) (by simp)
-           Kok ⬝ₒₖ (goto_okay Prok flt ⟨unpr_ok.concat ⟨glt, h⟩, prom_ok⟩
-                     (by rw[ρ.pushsig, getElem!_pos Pr.funs g glt']
-                         simp[BlockSig.spork] at bbody_ok; simp
-                         exact bbody_ok))
+    · case spork f K ρ X g g_args bbody wf =>
+       apply thread
+       exact match wf with
+         | Kwf ⬝wf ⟨flt, ⟨unpr_wf, prom_wf⟩, _, .code
+               (.spork glt gsig g_args_wf bbody_wf)⟩ =>
+           let glt' : g < P.funs.length := List.length_map (α := Func) (·.fsig) ▸ glt
+           let h : FuncSig.mk X[g_args]!.length P[g]!.fsig.ret = P.fsigs[g] :=
+             argsOfGetElem g_args_wf ▸
+             getElem!_pos P g glt' ▸
+             g_args_wf.map_length (λ x xwf => X[x]) ▸
+             gsig ▸
+             List.getElem_map (·.fsig) (l := P.funs) (h := glt) ▸
+             rfl
+           Kwf ⬝wf (.goto Pwf flt ⟨unpr_wf.concat ⟨glt, h⟩, prom_wf⟩
+                     (by rw[ρ.pushsig, getElem!_pos P g glt']
+                         simp at bbody_wf; simp
+                         exact bbody_wf))
 
-    · case promote f unpr g prom X K c K' u p ok =>
-        let kProm : K.allPromoted = true := by simp_all
+    · case promote f unpr g prom X K c K' u p wf =>
+        let kProm := CallStack.allPromoted_iff_nil.mpr u
         let rec hp : {K' : CallStack} -> {gets : Option Nat} -> K'.prom = [] ->
-                     CallStack.Okay Pr gets (K ⬝ ⟨f, ⟨g :: unpr, prom⟩, X, c⟩ ++ K') ->
-                     CallStack.Okay Pr gets (K ⬝ ⟨f, ⟨unpr, g.ret :: prom⟩, X, c⟩ ++ K') ∧
-                     CallStack.Okay Pr none {⟨g.f, ∅, g.args, codeEntry Pr g.f⟩} ∧
-                     g.ret = Pr.funs[g.f]!.fsig.ret
-          | .nil, gets, _, ok => by
+                     CallStack.WF P gets (K ⬝ ⟨f, ⟨g :: unpr, prom⟩, X, c⟩ ++ K') ->
+                     CallStack.WF P gets (K ⬝ ⟨f, ⟨unpr, g.ret :: prom⟩, X, c⟩ ++ K') ∧
+                     CallStack.WF P none {⟨g.f, ∅, g.args, .codeEntry P g.f⟩} ∧
+                     g.ret = P[g.f]!.fsig.ret
+          | .nil, gets, _, wf => by
             rw[CallStack.append_nil] at *
             apply And.intro <;> try (apply And.intro)
-            · exact ok.tail ⬝ₒₖ
-                (let kok := ok.head
-                 ⟨ok.head.flt,
-                  (let x := ok.head.ρₒₖ
+            · exact wf.tail ⬝wf
+                (let kwf := wf.head
+                 ⟨wf.head.flt,
+                  (let x := wf.head.ρwf
                    by rw[kProm] at *; exact x.promote),
-                  ok.head.cb,
-                  ok.head.cₒₖ⟩)
-            · apply (.nil ⬝ₒₖ ·)
-              let glt : g.f < Pr.funs.length := by
+                  wf.head.cb,
+                  wf.head.cwf⟩)
+            · apply (.nil ⬝wf ·)
+              let glt : g.f < P.funs.length := by
                 rw[← List.length_map (·.fsig)]
-                exact ok.head.ρₒₖ.unpr.head'.flt
-              let Prsize : Pr.funs.length = Pr.fsigs.length :=
-                (List.length_map (as := Pr.funs) (·.fsig)).symm
-              let glt' := Prsize ▸ glt
-              exact StackFrame.Okay.mk glt SpawnDeque.empty_okay rfl
-                (entry_okay (canProm := true) Prok glt
-                  (List.getElem_map Func.fsig (l := Pr.funs) ▸
-                   (congrArg (·.arity) ok.head.ρₒₖ.unpr.head'.sig).symm)
-                ).cₒₖ
-            · let gflt := ok.head.ρₒₖ.unpr.head'.flt
-              let gflt' : g.f < Pr.funs.length :=
-                List.length_map (as := Pr.funs) (·.fsig) ▸ gflt
-              let x : g.ret = Pr.fsigs[g.f].ret :=
-                congrArg (·.ret) ok.head.ρₒₖ.unpr.head'.sig
-              rw[getElem!_pos Pr.funs g.f gflt',
+                exact wf.head.ρwf.unpr.head'.flt
+              let Psize : P.funs.length = P.fsigs.length :=
+                (List.length_map (as := P.funs) (·.fsig)).symm
+              let glt' := Psize ▸ glt
+              exact StackFrame.WF.mk glt SpawnDeque.WF.empty rfl
+                (StackFrame.WF.entry (canProm := true) Pwf glt
+                  (List.getElem_map Func.fsig (l := P.funs) ▸
+                   (congrArg (·.arity) wf.head.ρwf.unpr.head'.sig).symm)
+                ).cwf
+            · let gflt := wf.head.ρwf.unpr.head'.flt
+              let gflt' : g.f < P.funs.length :=
+                List.length_map (as := P.funs) (·.fsig) ▸ gflt
+              let x : g.ret = P.fsigs[g.f].ret :=
+                congrArg (·.ret) wf.head.ρwf.unpr.head'.sig
+              rw[getElem!_pos P g.f gflt',
                  x,
-                 List.getElem_map (·.fsig) (l := Pr.funs)]
-          | K' ⬝ k', gets, p, ok =>
+                 List.getElem_map (·.fsig) (l := P.funs)]
+          | K' ⬝ k', gets, p, wf =>
             let ⟨kp', Kp'⟩ := List.append_eq_nil_iff.mp p
-            let k'ok := ok.head
-            let ⟨K'ok', gok, glt⟩ := hp Kp' ok.tail
-            let l := K'ok'
-            let k'ok' := k'ok.castCanProm
+            let k'wf := wf.head
+            let ⟨K'wf', gwf, glt⟩ := hp Kp' wf.tail
+            let l := K'wf'
+            let k'wf' := k'wf.castCanProm
               (K ⬝ ⟨f, ⟨unpr, g.ret :: prom⟩, X, c⟩ ++ K').allPromoted
               (λ (x : (K ⬝ ⟨f, ⟨g :: unpr, prom⟩, X, c⟩ ++ K').allPromoted) =>
                  let x' : (K ⬝ ⟨f, ⟨g :: unpr, prom⟩, X, c⟩ ++ K').unpr = [] :=
@@ -239,45 +188,33 @@ namespace Step
                    (List.append_eq_nil_iff.mp
                      (List.append_eq_nil_iff.mp
                        (CallStack.append_unpr ▸ x')).left).right
-                 by contradiction)
-            ⟨K'ok' ⬝ₒₖ k'ok', gok, glt⟩
-        let ⟨Kok, gok, glt⟩ := hp p ok
-        let prom_p : Pr.funs[g.f]!.fsig.ret ::
-                       (K ⬝ ⟨f, ⟨g :: unpr, prom⟩, X, c⟩ ++ K').prom =
-                     (K ⬝ ⟨f, ⟨unpr, g.ret :: prom⟩, X, c⟩ ++ K').prom := by
-          simp_all[CallStack.append_prom, p, glt]
-        exact cat (prom_p ▸ leaf Kok) (leaf gok)
+                 nomatch x'')
+            ⟨K'wf' ⬝wf k'wf', gwf, glt⟩
+        let ⟨Kwf, gwf, glt⟩ := hp p wf
+        exact node (thread Kwf) (thread gwf) (by simp_all) (by simp)
 
-    · case spoin_unpr f K ρ sc X bunpr bprom ok =>
-        apply @leaf Pr (K ⬝ ⟨f, ρ, X[bunpr.args]!, codeOf Pr f bunpr⟩)
-        exact match ok with
-          | Kok ⬝ₒₖ ⟨flt, ⟨unpr_ok, prom_ok⟩, _,
-              .code (.trfr (.spoin nn bunpr_ok bprom_ok))⟩ =>
+    · case spoin_unpr f K ρ sc X bunpr bprom wf =>
+        apply thread
+        exact match wf with
+          | Kwf ⬝wf ⟨flt, ⟨unpr_wf, prom_wf⟩, _,
+              .code (.spoin nn bunpr_wf bprom_wf)⟩ =>
             let h : (ρ.push sc).sig.tail = ρ.sig := by simp
-            Kok ⬝ₒₖ (goto_okay Prok flt ⟨unpr_ok.unconcat.1, prom_ok⟩ (h ▸ bunpr_ok))
+            Kwf ⬝wf (.goto Pwf flt ⟨unpr_wf.unconcat.1, prom_wf⟩ (h ▸ bunpr_wf))
 
-    · case spoin_prom f K ρ' X bunpr bprom Y y g K_unpr_nil retok ok =>
-        let g_ret_eq : g.ret = Pr.funs[g.f]!.fsig.ret :=
-          congrArg (λ | some x => x | _ => g.ret) (congrArg List.head? ok.same_prom)
-        let ρ_eq_ρ'_Kprom : ρ = ρ' ++ K.prom :=
-          Eq.symm (congrArg List.tail ok.same_prom)
-        rw[ρ_eq_ρ'_Kprom] at ok ⊢
-        apply @leaf Pr (K ⬝ ⟨f, ⟨[], ρ'⟩, X[bprom.args]! ++ Y[y]!, codeOf Pr f bprom⟩)
-        let ok'' : (ThreadPool.leaf (K ⬝ ⟨f, ⟨[], g.ret :: ρ'⟩, X,
-                      .code (.trfr (.spoin bunpr bprom))⟩)).Okay Pr (g.ret :: ρ' ++ K.prom) :=
-          g_ret_eq ▸ ok
-        let flt := ok''.get.head.flt
-        let sd_ok : (SpawnDeque.mk [] ρ').Okay Pr.fsigs K.allPromoted :=
-          ⟨IVec.nil, by simp[CallStack.allPromoted]; rw[K_unpr_nil]; rfl⟩
-        let y_ok : IVec (·.Okay Y.length) y :=
-          match retok.get.head.cₒₖ.c.t with
-            | .retn _ _ y_ok => y_ok
-        let y_len_eq_g_ret : y.length = g.ret :=
-          match retok.get.head.cₒₖ'.c.t with
-            | .retn _ l _ => g_ret_eq ▸ Eq.symm l
-        let cont_ok : bprom.OkayRets Pr.funs[f].bsigs ⟨X.length, ρ'⟩ y.length :=
-          match ok''.get.head.cₒₖ.c.t with
-            | .spoin nn unpr_ok prom_ok => y_len_eq_g_ret ▸ prom_ok
-        exact ok''.get.tail ⬝ₒₖ
-          (goto_okay_rets Prok flt sd_ok cont_ok y_ok)
+    · case spoin_prom f K ρ' X bunpr bprom Y y g K_unpr_nil wf retwf Rp R'p =>
+        let g_ret_eq : g.ret = P[g.f]!.fsig.ret :=
+          congrArg (λ | some x => x | _ => g.ret) R'p
+        apply thread
+        let wf'' : (ThreadTree.thread (K ⬝ ⟨f, ⟨[], g.ret :: ρ'⟩, X,
+                      .code (.spoin bunpr bprom)⟩)).WF P :=
+          g_ret_eq ▸ wf
+        let flt := wf''.get.head.flt
+        let sd_wf : (SpawnDeque.mk [] ρ').WF P.fsigs K.allPromoted :=
+          ⟨IVec.nil, by simp[K_unpr_nil]; rfl⟩
+        let y_wf : IVec (·.WF Y.length) y := retwf.get.head.cwf.c.retn_args
+        let y_len_eq_g_ret : y.length = g.ret := g_ret_eq ▸ retwf.get.head.cwf'.c.retn_length.symm
+        let cont_wf : bprom.WFRets P[f].bsigs ⟨X.length, ρ'⟩ y.length :=
+          y_len_eq_g_ret ▸ wf''.get.head.cwf.c.spoin_bprom
+        exact wf''.get.tail ⬝wf
+          (.goto_rets Pwf flt sd_wf cont_wf y_wf)
 end Step
